finished refactoring for circuit modulo performance and second part of filter

proof/correctness768/avx2/MLKEM_avx2_equivs.ec
@@ -20,7 +20,7 @@ require import MLKEM_Poly_avx2_proof.
 require import MLKEM_PolyVec_avx2_proof.
 require import MLKEM_Poly_avx2_vec.
 require import MLKEM_PolyVec_avx2_vec.
-require import MLKEM_InnerPKE.
+(* require import MLKEM_InnerPKE. *)
 require import MLKEMFCLib.
 
 import GFq Rq Symmetric Symmetric768 Serialization Serialization768 Sampling VecMat VecMat768 InnerPKE768 MLKEM768 Correctness768 Fq SignedReductions.
@@ -70,38 +70,28 @@ lemma poly_csubq_avx2_corr_h (_aw : W16.t Array256.t):
              pos_bound256_cxq res 0 256 1]. 
 proof.
 proc; inline *.
-proc change 1: (sliceget16_16_256 jqx16 0); 1: by auto.
-proc change ^while.1: (sliceget256_16_256 rp (i*256));1: by auto => /#.
-proc change ^while.9: (sliceset256_16_256 rp (i*256) r);1: by auto => /#.
-
+proc change 1: { qx16 <- sliceget16_16_256 jqx16 0;}; 1: by auto.
+proc change ^while.1: { r <- sliceget256_16_256 rp (i*256);};1: by auto => /#.
+proc change ^while.9: { rp <-sliceset256_16_256 rp (i*256) r;};1: by auto => /#.
 unroll for ^while.
 cfold ^i<-.
-wp -1. 
-bdep 16 16 [_aw] [rp] [rp] csubq_circuit pcond_reduced. 
+wp -1.
+conseq (: rp = _aw /\ all (fun c => W16.zero \sle c && c \slt W16.of_int 6658) rp ==>
+       rp = init_256_16 (fun i => csubq_circuit _aw.[i])); last by circuit.
 
+       
 (* BDEP pre conseq *)
-+ move => &hr />; rewrite flatten1 /= pre_lane_commute_in_aligned 1:/# //=.
-  rewrite allP /pos_bound768_cxq /= => Hb. 
-  rewrite /pcond_reduced /= /tolist /= => x.
-  rewrite  mkseqP => He;elim He => /= i [ib?]; rewrite ultE /=.
-  have := Hb i; rewrite ib /= qE /=.
-  rewrite /to_sint /smod /=.
-  smt(W16.to_uint_cmp).
++ move => &hr />. rewrite /pos_bound256_cxq /bpos16 qE /= => H.
+  rewrite /(\slt) /(\sle) /= /smod /= allP /=.
+  by exact H.
 
 (* BDEP post conseq *)
 
 (* We start with some boilerplate *)
-move => &hr [#]/= ->; rewrite /pos_bound256_cxq => Hb rr; rewrite /= !flatten1.
-rewrite !flattenK;1..4:smt(mapP W16.size_w2bits).
-rewrite -2!(map_comp) /(\o) /= -(map_comp W16.bits2w) /(\o).
-have -> := (eq_map (fun (x : W16.t) => W16.bits2w (w2bits x)) idfun);1: by move => ?/=/#.
-rewrite map_id.
-rewrite /lift_array256 /pos_bound256_cxq /= => H.
-rewrite -(Array256.to_listK witness rr) -H qE; split.
+move => &hr [#]/= ->; rewrite /pos_bound256_cxq => Hb rr; rewrite /init_256_16 /lift_array256 /= => ->; split.
 
 rewrite tP => i ib.
-rewrite !mapiE 1,2:/# /= get_of_list 1:/# (nth_map witness); 1:smt(Array256.size_to_list).
-rewrite (Array256.get_to_list _aw i).
+rewrite !mapiE 1,2:/# /= initiE 1:/# /=.
 rewrite /csubq_circuit ultE /W16_sub /=.
 move : (Hb i ib);rewrite /bpos16 qE /= /to_sint /smod /=.
 case (to_uint _aw.[i] < 3329) => *//;1:
@@ -110,10 +100,7 @@ rewrite to_uintB /=;1: by rewrite uleE => /#.
 have ->/= : !32768 <= to_uint _aw.[i] - 3329;  by smt(W16.to_uint_cmp).
 
 move => i ib.
-rewrite Array256.get_of_list 1:/# (nth_map witness); 1:smt(Array256.size_to_list).
-rewrite (nth_map witness) /=;1:smt(size_iota).
-rewrite nth_iota 1:/#.
-rewrite /csubq_circuit ultE /W16_sub /=.
+rewrite initiE 1:/# /= /csubq_circuit ultE /W16_sub /=.
 move : (Hb i ib);rewrite /bpos16 qE /= /to_sint /smod /=.
 case (to_uint _aw.[i] < 3329) => *//;1:
 have ->/= : !32768 <= to_uint _aw.[i] by smt(W16.to_uint_cmp).
@@ -139,40 +126,32 @@ lemma polyvec_csubq_avx2_corr_h (_aw : W16.t Array768.t):
              pos_bound768_cxq res 0 768 1]. 
 proof.
 proc; inline *.
-proc change ^while.1: (init_256_16 (fun i0 => r.[256*i+i0]));1: by auto.
-proc change ^while.2: (sliceget16_16_256 jqx16 0); 1: by auto.
-proc change ^while.^while.1: (sliceget256_16_256 rp (i0*256));1: by auto => /#.
-proc change ^while.^while.9: (sliceset256_16_256 rp (i0*256) r0);1: by auto => /#.
-proc change ^while.6: (init_768_16 (fun (i_0 : int) => if 256 * i <= i_0 < 256 * i + 256 then aux.[i_0 - 256 * i] else r.[i_0]));1: by auto. 
+proc change ^while.1: {rp <- init_256_16 (fun i0 => r.[256*i+i0]);};1: by auto.
+proc change ^while.2: {qx16 <- sliceget16_16_256 jqx16 0;}; 1: by auto.
+proc change ^while.^while.1: {r0 <- sliceget256_16_256 rp (i0*256);};1: by auto => /#.
+proc change ^while.^while.9: {rp <- sliceset256_16_256 rp (i0*256) r0;};1: by auto => /#.
+proc change ^while.6: {r <- init_768_16 (fun (i_0 : int) => if 256 * i <= i_0 < 256 * i + 256 then aux.[i_0 - 256 * i] else r.[i_0]);};1: by auto. 
 
 do 4!(unroll for ^while).
 cfold ^i0<-.
-wp -2. 
-bdep 16 16 [_aw] [r] [r] csubq_circuit pcond_reduced. 
+wp -2.
 
+conseq (: r = _aw /\ all (fun c => W16.zero \sle c && c \slt W16.of_int 6658) r ==>
+       r = init_768_16 (fun i => csubq_circuit _aw.[i])); last by circuit.
+
+       
 (* BDEP pre conseq *)
-+ move => &hr />; rewrite flatten1 /= pre_lane_commute_in_aligned 1:/# //=.
-  rewrite allP /pos_bound768_cxq /= => Hb. 
-  rewrite /pcond_reduced /= /tolist /= => x.
-  rewrite  mkseqP => He;elim He => /= i [ib?]; rewrite ultE /=.
-  have := Hb i; rewrite ib /= qE /=.
-  rewrite /to_sint /smod /=.
-  smt(W16.to_uint_cmp).
++ move => &hr />. rewrite /pos_bound768_cxq /bpos16 qE /= => H.
+  rewrite /(\slt) /(\sle) /= /smod /= allP /=.
+  by exact H.
 
 (* BDEP post conseq *)
 
 (* We start with some boilerplate *)
-move => &hr [#]/= ->; rewrite /pos_bound768_cxq => Hb rr; rewrite /= !flatten1.
-rewrite !flattenK;1..4:smt(mapP W16.size_w2bits).
-rewrite -2!(map_comp) /(\o) /= -(map_comp W16.bits2w) /(\o).
-have -> := (eq_map (fun (x : W16.t) => W16.bits2w (w2bits x)) idfun);1: by move => ?/=/#.
-rewrite map_id.
-rewrite /lift_array768 /pos_bound768_cxq /= => H.
-rewrite -(Array768.to_listK witness rr) -H qE; split.
+move => &hr [#]/= ->; rewrite /pos_bound256_cxq => Hb rr; rewrite  /= => ->; split.
 
 rewrite tP => i ib.
-rewrite !mapiE 1,2:/# /= get_of_list 1:/# (nth_map witness); 1:smt(Array768.size_to_list).
-rewrite (Array768.get_to_list _aw i).
+rewrite !mapiE 1,2:/# /= initiE 1:/# /=.
 rewrite /csubq_circuit ultE /W16_sub /=.
 move : (Hb i ib);rewrite /bpos16 qE /= /to_sint /smod /=.
 case (to_uint _aw.[i] < 3329) => *//;1:
@@ -181,10 +160,7 @@ rewrite to_uintB /=;1: by rewrite uleE => /#.
 have ->/= : !32768 <= to_uint _aw.[i] - 3329;  by smt(W16.to_uint_cmp).
 
 move => i ib.
-rewrite Array768.get_of_list 1:/# (nth_map witness); 1:smt(Array768.size_to_list).
-rewrite (nth_map witness) /=;1:smt(size_iota).
-rewrite nth_iota 1:/#.
-rewrite /csubq_circuit ultE /W16_sub /=.
+rewrite initiE 1:/# /= /csubq_circuit ultE /W16_sub /=.
 move : (Hb i ib);rewrite /bpos16 qE /= /to_sint /smod /=.
 case (to_uint _aw.[i] < 3329) => *//;1:
 have ->/= : !32768 <= to_uint _aw.[i] by smt(W16.to_uint_cmp).
@@ -211,198 +187,50 @@ lemma polyvec_decompress_ll :
 by proc;inline *;unroll for ^while; do 3!(cfold ^inc<-; unroll for ^while);auto.
 qed.
 (********** BEGIN BDEP PROOF OF DECOMPRESS **************)
-op decompress10_circuit(c : W10.t) : W16.t = 
-  truncateu16 (srl_32 (((zeroextu10_32 c) * W32.of_int 3329) + W32.of_int 512) (W32.of_int 10)).
-
-op pcond_true10(_: W10.t) = true.
-
-lemma init_id (rp0 : W8.t Array1088.t):
-  (Array960.init ("_.[_]" (Array960.init ("_.[_]" rp0)))) =
-    Array960.init  ("_.[_]" rp0).
-rewrite tP => *.
-by rewrite initiE 1:/# /=.
-qed.
 
 lemma polyvec_decompress_corr_h (_aw : W8.t Array960.t):
     hoare[ Jkem768_avx2.M.__i_polyvec_decompress :
              Array960.init (fun i => rp.[i]) = _aw ==> pos_bound768_cxq res 0 768 1 /\ lift_polyvec res = decompress_polyvec 10 (decode10_vec _aw)].
 proc; inline *.
-proc change 3: (sliceget32_8_256 pvd_shufbdidx_s 0); 1: by auto.
-proc change ^while.^while.1 : (sliceget1088_8_256 rp ((320*k + 20*i)*8)); 1: by auto => /> /#.
-proc change ^while.^while.8 : (sliceset768_16_256 r ((16 * k + i)*256) f); 1: by auto => /> /#.
+proc change 3: { shufbidx <- sliceget32_8_256 pvd_shufbdidx_s 0;}; 1: by auto.
+proc change ^while.^while.1 : {f <- sliceget1088_8_256 rp ((320*k + 20*i)*8);}; 1: by auto => /> /#.
+proc change ^while.^while.8 : {r <- sliceset768_16_256 r ((16 * k + i)*256) f;}; 1: by auto => /> /#.
 unroll for ^while.
 cfold ^inc<-.
 do 3!(unroll for ^while).
 cfold ^i<-.
 wp -3.
-bdep 10 16 [_aw[Array960.t:0]] [rp[Array960.t:0]] [r] decompress10_circuit pcond_true10. 
 
-(* BDEP pre conseq *)
-+ move => &hr />; rewrite /pcond_true10 /=;split. 
-  + rewrite allP /#. 
-  have {2}<- := init_id rp{hr}; smt().
 
-(* BDEP post conseq *)
-
+conseq (: rp = init_1088_8 (fun i => if i < 960 then _aw.[i] else rp.[i])
+        ==>
+   r = init_768_16 (fun i =>
+     decompress10_circuit (W10.init (fun (j : int) => _aw.[(i*10 + j) %/ 8].[(i*10 + j) %% 8]))));last  circuit. 
+     
 (* We start with some boilerplate *)
-move => &hr [#]/= <- rr; rewrite /= !flatten1.
-rewrite init_id.
-move => H1; have H2 := post_lane_commute_out_aligned (to_list (Array960.init ("_.[_]" rp{hr}))) (to_list rr) W8.w2bits W8.bits2w W10.w2bits W10.bits2w W16.w2bits W16.bits2w  decompress10_circuit 8 10 16 _ _ _ _ _ _ _ _ _ _ _ _ H1;1..12:
-smt(Array960.size_to_list Array768.size_to_list W16.bits2wK BVA_Top_Bindings_W10_t.oflistP).
+move => &hr /=;rewrite !tP  => H i ib.
+rewrite initiE /=;case (0 <= i < 960) => *; smt(Array960.initiE).
 
-have H3 : 
-   map decompress10_circuit (map W10.bits2w (chunk 10 (flatten (map W8.w2bits (to_list (Array960.init ("_.[_]" rp{hr}))))))) =
-   map (W16.of_int \o asint) (to_list (decompress_polyvec 10 (decode10_vec (Array960.init ("_.[_]" rp{hr})))).[0] ++ 
-                              to_list (decompress_polyvec 10 (decode10_vec (Array960.init ("_.[_]" rp{hr})))).[1] ++ 
-                              to_list (decompress_polyvec 10 (decode10_vec (Array960.init ("_.[_]" rp{hr})))).[2])%Vector.
-+ rewrite /decode10_vec /decompress_polyvec !map_cat !setvE !offunvE 1..3:/# /= !offunvK /vclamp /kvec /= /subarray256 /=.
-  apply (eq_from_nth witness).
-  + rewrite !size_map !size_cat !size_map !size_iota /max /=.
-     rewrite (EclibExtra.size_flatten' 8);1:smt(mapP W8.size_w2bits). 
-     by rewrite size_map size_to_list /=.
-  move => i.
-  rewrite !size_map size_iota.
-  rewrite (EclibExtra.size_flatten' 8);1:smt(mapP W8.size_w2bits). 
-   rewrite size_map size_to_list /max  /= => ib.
-  rewrite !nth_cat !size_map !size_cat !size_map !size_iota /max /=. 
-  case (i <256).
-  + move => ?;rewrite ifT 1:/#.
-    rewrite (nth_map witness).
-    + rewrite size_map size_chunk 1:/# (EclibExtra.size_flatten' 8);1:smt(mapP W8.size_w2bits). 
-      rewrite size_map size_to_list /= /#.
-    rewrite (nth_map []).
-    + rewrite  size_chunk 1:/# (EclibExtra.size_flatten' 8);1:smt(mapP W8.size_w2bits). 
-      rewrite size_map size_to_list /= /#.
-    rewrite (nth_map witness _ ((W16.of_int \o asint))) /=.
-    + rewrite size_to_list /= /#.
-   rewrite /(\o) /= mapiE 1:/# /= initiE 1:/# /=.  
-  rewrite /(\o) /decompress11_circuit -decompress_alt_decompress /decompress_alt //=.
-  rewrite get_of_list 1:/# /= qE /=.
-  have Hs := size_nth_chunk [] (flatten (map W8.w2bits (to_list(Array960.init ("_.[_]" rp{hr}))))) i 10 _ _ => //.
-  + rewrite (EclibExtra.size_flatten' 8);1:smt(mapP W8.size_w2bits). 
-    by rewrite size_map size_to_list /#.
-  rewrite to_uint_eq to_uint_truncateu16 /= /srl_32 /= of_uintK /=;congr;congr.
-  have ? : 2^10 = 1024 by auto.
-  rewrite to_uint_shr //= /zeroextu10_32 to_uintD_small /=;1: by rewrite of_uintK /=; smt(modz_small W10.to_uint_cmp). 
-  rewrite of_uintK /= modz_small /=;1:by smt( W10.to_uint_cmp). 
-  rewrite /to_uint bits2wK 1:/# incoeffK qE /= /decode (nth_map [] _ bs2int) /=.
-  + rewrite size_chunk 1:/# size_BytesToBits size_to_list /= /#.
-  by smt(BS2Int.bs2int_ge0 BS2Int.bs2int_le2Xs modz_small W10.to_uint_cmp). 
+move => &hr <- rr ->; split; last first.
++ rewrite eq_vectorP => k kb.
+  rewrite tP => i ib.
+  rewrite /lift_polyvec /init_768_16 offunvE 1:/# /= !mapiE 1:/# /= -get_to_list /= initiE 1:/# /= initiE 1:/# /=.
+  rewrite /decompress10_circuit decompress10_circuit_sem 1:/# /=.
+  rewrite /decompress_polyvec /= !setvE /= offunvE 1:/# /=.
+  case (2 = k) => ?; 1: 
+   by rewrite mapiE 1:/# /= /subarray256 initiE 1:/# /= initiE 1:/# /= /decode10_vec get_of_list /#.
+  rewrite offunvK /vclamp kb /=.
+  case (1 = k) => ?; 1: 
+   by rewrite mapiE 1:/# /= /subarray256 initiE 1:/# /= initiE 1:/# /= /decode10_vec get_of_list /#.
+  rewrite offunvK /vclamp kb /=.
+  by rewrite ifT 1:/# mapiE 1:/# /= /subarray256 initiE 1:/# /= initiE 1:/# /= /decode10_vec get_of_list /#.
 
-  case (i <512).
-  + move => ??.
-    rewrite (nth_map witness).
-    + rewrite size_map size_chunk 1:/# (EclibExtra.size_flatten' 8);1:smt(mapP W8.size_w2bits). 
-      rewrite size_map size_to_list /= /#.
-    rewrite (nth_map []).
-    + rewrite  size_chunk 1:/# (EclibExtra.size_flatten' 8);1:smt(mapP W8.size_w2bits). 
-      rewrite size_map size_to_list /= /#.
-    rewrite (nth_map witness _ ((W16.of_int \o asint))) /=.
-    + rewrite size_to_list /= /#.
-   rewrite /(\o) /= mapiE 1:/# /= initiE 1:/# /=.  
-  rewrite /(\o) /decompress11_circuit -decompress_alt_decompress /decompress_alt //=.
-  rewrite get_of_list 1:/# /= qE /=.
-  have Hs := size_nth_chunk [] (flatten (map W8.w2bits (to_list (Array960.init ("_.[_]" rp{hr}))))) i 10 _ _ => //.
-  + rewrite (EclibExtra.size_flatten' 8);1:smt(mapP W8.size_w2bits). 
-    by rewrite size_map size_to_list /#.
-  rewrite to_uint_eq to_uint_truncateu16 /= /srl_32 /= of_uintK /=;congr;congr.
-  have ? : 2^10 = 1024 by auto.
-  rewrite to_uint_shr //= /zeroextu10_32 to_uintD_small /=;1: by rewrite of_uintK /=; smt(modz_small W10.to_uint_cmp). 
-  rewrite of_uintK /= modz_small;1:by smt( W10.to_uint_cmp). 
-  rewrite /to_uint bits2wK 1:/# incoeffK qE /= /decode (nth_map [] _ bs2int) /=.
-  + rewrite size_chunk 1:/# size_BytesToBits size_to_list /= /#.
-  by smt(BS2Int.bs2int_ge0 BS2Int.bs2int_le2Xs modz_small W10.to_uint_cmp). 
-
-  + move => ??.
-    rewrite (nth_map witness).
-    + rewrite size_map size_chunk 1:/# (EclibExtra.size_flatten' 8);1:smt(mapP W8.size_w2bits). 
-      rewrite size_map size_to_list /= /#.
-    rewrite (nth_map []).
-    + rewrite  size_chunk 1:/# (EclibExtra.size_flatten' 8);1:smt(mapP W8.size_w2bits). 
-      rewrite size_map size_to_list /= /#.
-    rewrite (nth_map witness _ ((W16.of_int \o asint))) /=.
-    + rewrite size_to_list /= /#.
-   rewrite /(\o) /= mapiE 1:/# /= initiE 1:/# /=.  
-  rewrite /(\o) /decompress11_circuit -decompress_alt_decompress /decompress_alt //=.
-  rewrite get_of_list 1:/# /= qE /=.
-  have Hs := size_nth_chunk [] (flatten (map W8.w2bits (to_list (Array960.init ("_.[_]" rp{hr}))))) i 10 _ _ => //.
-  + rewrite (EclibExtra.size_flatten' 8);1:smt(mapP W8.size_w2bits). 
-    by rewrite size_map size_to_list /#.
-  rewrite to_uint_eq to_uint_truncateu16 /= /srl_32 /= of_uintK /=;congr;congr.
-  have ? : 2^10 = 1024 by auto.
-  rewrite to_uint_shr //= /zeroextu10_32 to_uintD_small /=;1: by rewrite of_uintK /=; smt(modz_small W10.to_uint_cmp). 
-  rewrite of_uintK /= modz_small;1:by smt( W10.to_uint_cmp). 
-  rewrite /to_uint bits2wK 1:/# incoeffK qE /= /decode (nth_map [] _ bs2int) /=.
-  + rewrite size_chunk 1:/# size_BytesToBits size_to_list /= /#.
-  by smt(BS2Int.bs2int_ge0 BS2Int.bs2int_le2Xs modz_small W10.to_uint_cmp). 
-
-
-split; last first.
-+ rewrite eq_vectorP => i @/kvec ib.
-  rewrite /lift_polyvec /decompress_polyvec !setvE !offunvE 1..2:/# /= !offunvK /vclamp /kvec /= ib /=. 
-
-  case (2 = i) => Hi2.
-  + rewrite tP => k kb. 
-    rewrite -Hi2 !mapiE 1,2:/# !initiE 1,2:/# /= /= -get_to_list H2 H3 /(\o) /=.
-  rewrite (nth_map witness) /=;1: by smt(Array256.size_to_list size_cat).
-  rewrite (nth_cat witness).
-  + rewrite !size_cat !size_to_list /= ifF 1:/# /decompress_polyvec.
-    rewrite !setvE !offunvE 1:/# /=.
-  rewrite get_of_list 1:/# /decode10_vec mapiE 1:/# /= initiE 1:/# /= get_of_list 1:/# /= /smod /=.
-  pose c := decompress 10 (nth 0 (decode 10 (to_list (Array960.init ("_.[_]" rp{hr})))) (512 + k)).
-  rewrite modz_small; smt(@Zq).  
-
-  case (1 = i) => Hi1.
-  + rewrite tP => k kb. 
-    rewrite -Hi1 !mapiE 1,2:/# !initiE 1,2:/# /= /= -get_to_list H2 H3 /(\o) /=.
-  rewrite (nth_map witness) /=;1: by smt(Array256.size_to_list size_cat).
-  rewrite (nth_cat witness).
-  + rewrite !size_cat !size_to_list /= ifT 1:/# /decompress_polyvec.
-    rewrite !setvE !offunvE 1,2:/# /= !offunvK /vclamp /= !ifT 1..3:/#.
-  rewrite (nth_cat witness).
-  + rewrite !size_to_list /= ifF 1:/# /decompress_polyvec.
-  rewrite get_of_list 1:/# /decode10_vec mapiE 1:/# /= initiE 1:/# /= get_of_list 1:/# /= /smod /=.
-  pose c := decompress 10 (nth 0 (decode 10 (to_list (Array960.init ("_.[_]" rp{hr})))) (256 + k)).
-  rewrite modz_small; smt(@Zq).  
-
-
-  have Hi0 :(0 = i) by smt().
-  + rewrite tP => k kb.
-    rewrite -Hi0 /= !mapiE 1,2:/# /= initiE 1:/# /= -( Array768.get_to_list rr) H2 H3.
-  rewrite (nth_map witness);1: by smt(Array256.size_to_list size_cat).
-  rewrite (nth_cat witness).
-  + rewrite !size_cat !size_to_list /= ifT 1:/# /decompress_polyvec.
-    rewrite !setvE !offunvE 1..2:/# /= !offunvK /vclamp /= !ifT 1..3:/#.
-  rewrite (nth_cat witness).
-  + rewrite  !size_to_list /= ifT 1:/# /decompress_polyvec.
-    rewrite  mapiE 1:/# initiE 1:/# /= initiE 1:/# /=.
-    rewrite of_sintK /= /smod /= ifF;1:smt(@Zq).
-    pose c := (decompress 10 (nth 0 (decode 10 (to_list (Array960.init ("_.[_]" rp{hr})))) (k))).
-  rewrite modz_small; smt(@Zq).  
-
-
+  
 rewrite /pos_bound768_cxq qE /= => k kb. 
-rewrite -get_to_list  H2 H3 /decompress_poly.
-rewrite (nth_map witness);1: by smt(size_cat Array256.size_to_list).
-rewrite (nth_cat witness) !size_cat !size_to_list /=. 
-rewrite (nth_cat witness)  !size_to_list /=. 
-rewrite /decompress_polyvec !setvE /= !offunvE 1..3:/# /= !offunvK /= /vclamp /kvec/=.
-case (k < 256).
-+ move => *; rewrite ifT 1:/# .
-  rewrite mapiE 1:/# initiE 1:/# /=.
-  rewrite of_sintK /= /smod /= ifF;1:smt(@Zq).
-  rewrite modz_small; smt(@Zq).  
-case (k < 512).
-+ move => *.
-  rewrite mapiE 1:/# initiE 1:/# /=.
-  rewrite of_sintK /= /smod /= ifF;1:smt(@Zq).
-  rewrite modz_small; smt(@Zq).  
-+ move => *.
-  rewrite mapiE 1:/# initiE 1:/# /=.
-  rewrite of_sintK /= /smod /= ifF;1:smt(@Zq).
-  rewrite modz_small; smt(@Zq).  
-
+rewrite /init_768_16 initiE 1:/# /=.
+by apply decompress10_circuit_rng.
 qed.
+
 
 
 lemma polyvec_decompress_corr (_aw : W8.t Array960.t):
@@ -442,11 +270,6 @@ qed.
 
 
 (********** BEGIN BDEP PROOF OF COMPRESS  **************)
-op compress10_circuit(a : W16.t) : W10.t = 
-   if (a \ult W16.of_int 3329) then  
-   truncate64_10 (srl_64 ((sll_64 (zeroextu64 a) (W64.of_int 10) + W64.of_int 1665) * W64.of_int 1290167) (W64.of_int 32))
-   else 
-   truncate64_10 (srl_64 ((sll_64 (zeroextu64 (W16_sub a (W16.of_int 3329))) (W64.of_int 10) + W64.of_int 1665) * W64.of_int 1290167) (W64.of_int 32)).
 
 abbrev keepodd10 = (W32.of_int 67043328).
 abbrev keepeven10 = (W32.of_int 1023).
@@ -735,17 +558,17 @@ lemma auxcompress10_corr_h (_aw : W16.t Array768.t):
       res = encode10_vec (compress_polyvec 10 (lift_polyvec _aw))].
 proof.
 proc; inline *.
-proc change ^while.1: (init_256_16 (fun i => r.[256*i0+i]));1: by auto.
-proc change ^while.2: (sliceget16_16_256 jqx16 0); 1: by auto.
-proc change ^while.^while.1: (sliceget256_16_256 rp0 (i1*256));1: by auto => /#.
-proc change ^while.^while.9: (sliceset256_16_256 rp0 (i1*256) r0);1: by auto => /#.
-proc change ^while.6: (init_768_16 (fun (i_0 : int) => if 256 * i0 <= i_0 < 256 * i0 + 256 then aux.[i_0 - 256 * i0] else r.[i_0]));1: by auto. 
-proc change 7: (sliceget16_16_256 x16p 0); 1: by auto.
-proc change ^while{2}.1: (sliceget768_16_256 a (i*256));1: by auto => /#.
-proc change 14: (sliceget32_8_256 pvc_shufbidx_s 0); 1: by auto.
-proc change ^while{2}.19 : (sliceset960_8_128 rp  (20*i*8) t0);1: by auto => /#.
-proc change ^while{2}.20 : (sliceset960_8_32 rp  ((20*i+16)*8) (truncateu32 t1)).
-+ move => *;rewrite /sliceset960_8_32 tP => *.
+proc change ^while.1: { rp0 <- init_256_16 (fun i => r.[256*i0+i]);};1: by auto.
+proc change ^while.2: { qx16 <- sliceget16_16_256 jqx16 0;}; 1: by auto.
+proc change ^while.^while.1: {r0 <- sliceget256_16_256 rp0 (i1*256);};1: by auto => /#.
+proc change ^while.^while.9: { rp0 <- sliceset256_16_256 rp0 (i1*256) r0;};1: by auto => /#.
+proc change ^while.6: { r <- init_768_16 (fun (i_0 : int) => if 256 * i0 <= i_0 < 256 * i0 + 256 then aux.[i_0 - 256 * i0] else r.[i_0]);};1: by auto. 
+proc change 7: { v <- sliceget16_16_256 x16p 0;}; 1: by auto.
+proc change ^while{2}.1: {f0 <- sliceget768_16_256 a (i*256);};1: by auto => /#.
+proc change 14: { shufbidx <- sliceget32_8_256 pvc_shufbidx_s 0;}; 1: by auto.
+proc change ^while{2}.19 : { rp <- sliceset960_8_128 rp  (20*i*8) t0;};1: by auto => /#.
+proc change ^while{2}.20 : { rp <- sliceset960_8_32 rp  ((20*i+16)*8) (truncateu32 t1);}.
++ auto => />;move => *;rewrite /sliceset960_8_32 tP => *.
   rewrite initiE /= 1:/# ifT 1:/# initiE 1:/#.
   do congr;1: smt(). 
   by rewrite /VPEXTR_32 /truncateu32 to_uint_eq /= bits32_div //.
@@ -755,123 +578,30 @@ cfold ^inc<-.
 unroll for ^while.
 cfold ^i0<-. 
 cfold ^i1<-. 
-wp -4. 
-bdep 16 10 [_aw] [a] [rp] compress10_circuit pcond_reduced. 
+wp -4.
 
+conseq (: a = _aw /\
+   Array768.all (fun bv => W16.zero \sle bv /\ bv \slt (of_int (2 * 3329))) a
+   ==> rp = init_960_8 (fun i =>
+     W8.init (fun j =>
+       (compress10_circuit _aw.[(i*8+j) %/ 10]).[(i*8+j) %% 10]))); last by admit.   (* FIXME TAKES TOO LONG! by circuit *)
 
+      
 (* BDEP pre conseq *)
-+ move => &hr />; rewrite flatten1 /= pre_lane_commute_in_aligned 1:/# //=.
-  rewrite allP /pos_bound768_cxq /= => Hb. 
-  rewrite /pcond_reduced /= /tolist /= => x.
-  rewrite  mkseqP => He;elim He => /= i [ib?]; rewrite ultE /=.
-  have := Hb i; rewrite ib /= qE /=.
-  rewrite /to_sint /smod /=.
-  smt(W16.to_uint_cmp).
-
++ move => &hr />; rewrite /pos_bound768_cxq qE /= /(\sle) /(\slt) allP /=  => Hb i ib /=.
+  rewrite /(to_sint W16.zero) /= /(W16.smod 0) /=.
+  rewrite /(to_sint (W16.of_int 6658)) /= /(W16.smod 6658) /= /#.
+  
 (* BDEP post conseq *)
 
 (* We start with some boilerplate *)
-move => &hr [#]/= <- H0  rr; rewrite /= !flatten1.
-move => H1.
-
-apply (inj_eq Array960.to_list Array960.to_list_inj).
-apply (flatten_map_eq _ _ W8.w2bits 8 _ W8.w2bits_inj W8.size_w2bits);1:smt().
-have -> := post_lane_commute_in_aligned (to_list a{hr}) (to_list rr) W16.w2bits W16.bits2w W8.w2bits W8.bits2w W10.w2bits W10.bits2w  compress10_circuit 16 10 8 _ _ _ _ _ _ _ _ _ _ _ _ H1;1..12:
-    smt(Array960.size_to_list Array768.size_to_list W16.bits2wK BVA_Top_Bindings_W10_t.oflistP).
-
-rewrite output_pack_960_8. 
-+ rewrite (EclibExtra.size_flatten' 10);1: smt(mapP BS2Int.size_int2bs).
-  by rewrite size_map size_to_list /=.
-
-congr.
-rewrite /compress10_circuit /compress_polyvec /fromarray256  -map_comp -map_comp -map_comp /(\o) /=.  
-apply (eq_from_nth witness); 1: by rewrite !size_map //.
-rewrite size_map size_iota /max /= => i ib; rewrite !(nth_map witness) //=;1,2:smt(size_iota).
-rewrite nth_iota 1:/# mapiE 1:/# initiE 1:/# /= /lift_polyvec /=.
-case (0<=i<256).
-+ move => ? /=.
-  rewrite  !getvE offunvE 1:/# /= -(BVA_Top_Bindings_W10_t.oflistP (int2bs 10 (compress 10 (lift_array256 (subarray256 a{hr} 0)).[i]))); 1: by rewrite BS2Int.size_int2bs /#.
-congr; rewrite -BVA_Top_Bindings_W10_t.ofintP /lift_array256 /subarray256 !mapiE 1:/# /= initiE 1:/# /=. 
-
-rewrite /truncate64_10 to_uint_eq.
-(* This is now the equivalence betwen specs. It's made slightly more verbose
-   because the impl circuit is only proved correct wrt compress for values
-   in the q range. *)
-rewrite ultE /=. 
-case (to_uint a{hr}.[i] < 3329) => /= *.
-+ rewrite -Fq.compress_impl_large //=; 1: by rewrite /bpos16 qE /= /to_sint /smod /=;smt(W16.to_uint_cmp).     
-  rewrite /srl_64 /sll_64 /(`<<`) /(`>>`) !of_uintK /= /#. 
-have := H0;rewrite /pos_bound768_cxq qE /= => H00.
-
-have ? : 0 <= to_sint ((W16_sub a{hr}.[i] (W16.of_int 3329))) < 3329.
-+  rewrite /bpos16 to_sintB_small /=;1: by rewrite  /(to_sint (W16.of_int 3329)) /smod /= /smod /=;smt(size_map size_iota). 
-   by rewrite  /(to_sint (W16.of_int 3329)) /smod /=; smt(size_map size_iota W16.to_uint_cmp).
-
-have ? : to_sint ((W16_sub a{hr}.[i] (W16.of_int 3329))) = to_sint a{hr}.[i] -  3329.
-+  rewrite to_sintB_small /=;1: by rewrite  /(to_sint (W16.of_int 3329)) /= /smod /=;smt(size_map size_iota). 
-   by rewrite  /(to_sint (W16.of_int 3329)) /= /smod /=; smt(size_map size_iota W16.to_uint_cmp).
-
-have -> : (incoeff (to_sint a{hr}.[i])) = (incoeff (to_sint (W16_sub a{hr}.[i] (W16.of_int 3329)))) by  rewrite -eq_incoeff;  smt().  
-
-rewrite -Fq.compress_impl_large //=;1:by smt().
-by rewrite /srl_64 /sll_64 /(`<<`) /(`>>`) !of_uintK /= /#. 
-
-case (256<=i<512).
-+ move => ?? /=.
-  rewrite  !getvE offunvE 1:/# /= -(BVA_Top_Bindings_W10_t.oflistP (int2bs 10 (compress 10 (lift_array256 (subarray256 a{hr} 1)).[i-256]))); 1: by rewrite BS2Int.size_int2bs /#.
-congr; rewrite -BVA_Top_Bindings_W10_t.ofintP /lift_array256 /subarray256 !mapiE 1:/# /= initiE 1:/# /=. 
-
-rewrite /truncate64_11 to_uint_eq.
-(* This is now the equivalence betwen specs. It's made slightly more verbose
-   because the impl circuit is only proved correct wrt compress for values
-   in the q range. *)
-rewrite ultE /=. 
-case (to_uint a{hr}.[i] < 3329) => /= *.
-+ rewrite -Fq.compress_impl_large //=; 1: by rewrite /bpos16 qE /= /to_sint /smod /=;smt(W16.to_uint_cmp).     
-  rewrite /srl_64 /sll_64 /(`<<`) /(`>>`) !of_uintK /= /#. 
-have := H0;rewrite /pos_bound768_cxq qE /= => H00.
-
-have ? : 0 <= to_sint ((W16_sub a{hr}.[i] (W16.of_int 3329))) < 3329.
-+  rewrite /bpos16 to_sintB_small /=;1: by rewrite  /(to_sint (W16.of_int 3329)) /= /smod /=;smt(size_map size_iota). 
-   by rewrite  /(to_sint (W16.of_int 3329))   /= /smod /=; smt(size_map size_iota W16.to_uint_cmp).
-
-have ? : to_sint ((W16_sub a{hr}.[i] (W16.of_int 3329))) = to_sint a{hr}.[i] -  3329.
-+  rewrite to_sintB_small /=;1: by rewrite  /(to_sint (W16.of_int 3329))  /= /smod /=;smt(size_map size_iota). 
-   by rewrite  /(to_sint (W16.of_int 3329))  /= /smod /=; smt(size_map size_iota W16.to_uint_cmp).
-
-have -> : (incoeff (to_sint a{hr}.[i])) = (incoeff (to_sint (W16_sub a{hr}.[i] (W16.of_int 3329)))) by  rewrite -eq_incoeff;  smt().  
-
-rewrite -Fq.compress_impl_large //=;1:by smt().
-by rewrite /srl_64 /sll_64 /(`<<`) /(`>>`) !of_uintK /= /#. 
-
-+ move => ?? /=.
-  rewrite  !getvE offunvE 1:/# /= -(BVA_Top_Bindings_W10_t.oflistP (int2bs 10 (compress 10 (lift_array256 (subarray256 a{hr} 2)).[i-512]))); 1: by rewrite BS2Int.size_int2bs /#.
-congr; rewrite -BVA_Top_Bindings_W10_t.ofintP /lift_array256 /subarray256 !mapiE 1:/# /= initiE 1:/# /=. 
-
-rewrite /truncate64_10 to_uint_eq.
-(* This is now the equivalence betwen specs. It's made slightly more verbose
-   because the impl circuit is only proved correct wrt compress for values
-   in the q range. *)
-rewrite ultE /=. 
-case (to_uint a{hr}.[i] < 3329) => /= *.
-+ rewrite -Fq.compress_impl_large //=; 1: by rewrite /bpos16 qE /= /to_sint /smod /=;smt(W16.to_uint_cmp).     
-  rewrite /srl_64 /sll_64 /(`<<`) /(`>>`) !of_uintK /= /#. 
-have := H0;rewrite /pos_bound768_cxq qE /= => H00.
-
-have ? : 0 <= to_sint ((W16_sub a{hr}.[i] (W16.of_int 3329))) < 3329.
-+  rewrite /bpos16 to_sintB_small /=;1: by rewrite  /(to_sint (W16.of_int 3329)) /= /smod /=;smt(size_map size_iota). 
-   by rewrite  /(to_sint (W16.of_int 3329)) /= /smod /=; smt(size_map size_iota W16.to_uint_cmp).
-
-have ? : to_sint ((W16_sub a{hr}.[i] (W16.of_int 3329))) = to_sint a{hr}.[i] -  3329.
-+  rewrite to_sintB_small /=;1: by rewrite  /(to_sint (W16.of_int 3329)) /= /smod /=;smt(size_map size_iota). 
-   by rewrite  /(to_sint (W16.of_int 3329))  /= /smod /=; smt(size_map size_iota W16.to_uint_cmp).
-
-have -> : (incoeff (to_sint a{hr}.[i])) = (incoeff (to_sint (W16_sub a{hr}.[i] (W16.of_int 3329)))) by  rewrite -eq_incoeff;  smt().  
-
-rewrite -Fq.compress_impl_large //=;1:by smt().
-by rewrite /srl_64 /sll_64 /(`<<`) /(`>>`) !of_uintK /= /#. 
-
+move => &hr [#]/= -> H0 rr; rewrite /= /init_960_8 !tP => H i ib.
+rewrite H // initiE 1:/# /=.
+rewrite wordP => k kb; rewrite !initiE /= 1,2:/#.
+rewrite encode_vec_compress_bits //=.
+by apply compress10_circuit_sem.
 qed.
+
 (********** END BDEP PROOF OF COMPRESS **************)
 
 lemma auxcompress10_corr (_aw : W16.t Array768.t):
@@ -956,10 +686,6 @@ qed.
 
 (********** BEGIN BDEP PROOF OF DECOMPRESS **************)
 
-op decompress4_circuit(c : W4.t) : W16.t =
-  truncateu16 (srl_32 (((zeroextu4_32 c) * W32.of_int 3329) + W32.of_int 8) (W32.of_int 4)).
-
-op pcond_true4(_: W4.t) = true.
 
 lemma poly_decompress_ll : islossless Jkem768_avx2.M._i_poly_decompress.
  proc; inline *;wp. cfold 9; unroll for ^while;auto.
@@ -972,62 +698,32 @@ lemma poly_decompress_corr_h (_a : W8.t Array128.t):
              lift_array256 res = decompress_poly 4 (decode4 _a) /\
              pos_bound256_cxq res 0 256 1 ].
 proc; inline *.
-proc change 4: (sliceget16_16_256 x16p 0); 1: by auto.
-proc change 6: (sliceget32_8_256 x32p 0); 1: by auto.
-proc change ^while.1 : (zeroextu128 (sliceget128_8_64 a ((8*i)*8)));1: by auto => /#.
-proc change ^while.8 : (sliceset256_16_256 rp (i*256) f);1: by auto => /#.
+proc change 4: { q <- sliceget16_16_256 x16p 0;}; 1: by auto.
+proc change 6: { shufbidx <- sliceget32_8_256 x32p 0;}; 1: by auto.
+proc change ^while.1 : { h <- zeroextu128 (sliceget128_8_64 a ((8*i)*8));};1: by auto => /#.
+proc change ^while.8 : { rp <- sliceset256_16_256 rp (i*256) f;};1: by auto => /#.
 
 cfold 9.
 unroll for ^while.
 cfold ^i<-.
 wp -2.
+conseq (: _ ==> rp = init_256_16 (fun i =>
+     decompress4_circuit (W4.init (fun (j : int) => _a.[i %/ 2].[i %% 2 * 4 + j])))); last  by circuit.
 
-bdep 4 16 [_a] [a] [rp] decompress4_circuit pcond_true4. 
-
-(* BDEP pre conseq *)
-+ by move => &hr />; rewrite allP /pcond_true4 /=. 
-
-(* BDEP post conseq *)
-
+      
 (* We start with some boilerplate *)
-move => &hr [#]/= <- rr; rewrite /= !flatten1.
-move => H1; have H2 := post_lane_commute_out_aligned (to_list a{hr}) (to_list rr) W8.w2bits W8.bits2w W4.w2bits W4.bits2w W16.w2bits W16.bits2w  decompress4_circuit 8 4 16 _ _ _ _ _ _ _ _ _ _ _ _ H1;1..12:
-smt(Array128.size_to_list Array256.size_to_list W16.bits2wK BVA_Top_Bindings_W4_t.oflistP).
-
-have H3 : 
-   map decompress4_circuit (map W4.bits2w (chunk 4 (flatten (map W8.w2bits (to_list a{hr}))))) =
-   map (W16.of_int \o asint) (to_list (decompress_poly 4 (decode4 a{hr}))).
-+ rewrite /decode4 /decompress_poly Array256.map_of_list Array256.of_listK;1:smt(size_map Array256.size_to_list).
-  rewrite /decode -map_comp  -(map_comp _ (decompress 4)) -(map_comp _ BS2Int.bs2int) /=.
-  apply eq_in_map => x xb. 
-  rewrite /(\o) /decompress4_circuit  -decompress_alt_decompress /decompress_alt //=.
-  have := size_nth_chunk [] (flatten (map W8.w2bits (to_list a{hr}))).
-  have := nthP witness (chunk 4 (flatten (map W8.w2bits (to_list a{hr})))) x.
-  rewrite xb /= => He;elim He; rewrite size_chunk //= => k*. 
-  have ? : size x = 4
-   by  have := size_nth_chunk witness (flatten (map W8.w2bits (to_list a{hr}))) k 4 =>/= /#.
-  rewrite qE to_uint_eq to_uint_truncateu16 /= /srl_32 /= of_uintK /=;congr;congr.
-  rewrite to_uint_shr //= /zeroextu4_32 to_uintD_small /=;1: by rewrite of_uintK /=;smt(modz_small W4.to_uint_cmp pow2_4). 
-  rewrite of_uintK /= modz_small;1:by smt( W4.to_uint_cmp pow2_4). 
-  rewrite /to_uint bits2wK 1:/# incoeffK qE /=. 
-  by smt(BS2Int.bs2int_ge0 BS2Int.bs2int_le2Xs modz_small W4.to_uint_cmp pow2_4). 
+move => &hr [#]/= <- rr /= ->.
 
 split.
 + rewrite tP => i ib.
-  rewrite !mapiE 1,2:/# /= -get_to_list H2 H3 /decompress_poly.
-  rewrite (nth_map witness);1: by smt(Array256.size_to_list).
-  rewrite get_to_list /= /(\o) mapiE 1:/# /=.
-  pose c := (decompress 4 (decode4 a{hr}).[i]).
-  rewrite  /smod /= ifF;1:smt(@Zq).
-  rewrite modz_small; smt(@Zq).  
+  rewrite /init_256_16 !mapiE 1,2:/# /= -get_to_list /= initiE 1:/# /=.
+  by rewrite  -decompress4_circuit_sem 1:/# /=. 
 
 rewrite /pos_bound256_cxq qE /= => k kb. 
-rewrite -get_to_list  H2 H3 /decompress_poly.
-  rewrite (nth_map witness);1: by smt(Array256.size_to_list).
-  rewrite get_to_list /= /(\o) mapiE 1:/# /=.
-  rewrite/= /smod /= ifF;1:smt(@Zq).
-  rewrite modz_small; smt(@Zq).  
+rewrite /init_256_16 initiE 1:/# /=.
+by apply decompress4_circuit_rng.
 qed.
+
 (********** END BDEP PROOF OF DECOMPRESS **************)
 
 lemma poly_decompress_corr (_a : W8.t Array128.t): 
@@ -1056,12 +752,6 @@ qed.
 
 
 (********** BEGIN BDEP PROOF OF COMPRESS  **************)
-print compress_alt.
-op compress4_circuit(a : W16.t) : W4.t = 
-   if (a \ult W16.of_int 3329) then  
-   truncateu32_4 (srl_32 ((sll_32 (zeroextu32 a) (W32.of_int 4) + W32.of_int 1665) * W32.of_int 80635) (W32.of_int 28))
-   else 
-   truncateu32_4 (srl_32 ((sll_32 (zeroextu32 (W16_sub a (W16.of_int 3329))) (W32.of_int 4) + W32.of_int 1665) * W32.of_int 80635) (W32.of_int 28)).  
 
 lemma i_poly_compress_corr_ll : islossless Jkem768_avx2.M._i_poly_compress.
 proof.
@@ -1080,78 +770,43 @@ lemma i_poly_compress_corr_h _aw  :
              ].
 proof.
 proc; inline *.
-proc change 3: (sliceget16_16_256 jqx16 0); 1: by auto.
-proc change ^while.1: (sliceget256_16_256 rp0 (i0*256));1: by auto => /#.
-proc change ^while.9: (sliceset256_16_256 rp0 (i0*256) r);1: by auto => /#.
-proc change 8: (sliceget16_16_256 x16p 0); 1: by auto.
-proc change 12: (sliceget8_32_256 pc_permidx_s 0); 1: by auto.
-proc change ^while{2}.1: (sliceget256_16_256 a (4*i*256));1: by auto => /#.
-proc change ^while{2}.2: (sliceget256_16_256 a ((4*i+1)*256));1: by auto => /#.
-proc change ^while{2}.3: (sliceget256_16_256 a ((4*i+2)*256));1: by auto => /#.
-proc change ^while{2}.4: (sliceget256_16_256 a ((4*i+3)*256));1: by auto => /#.
-proc change ^while{2}.23 : (sliceset128_8_256 rp  (32*i*8) f0);1: by auto => /#.
+proc change 3: { qx16 <- sliceget16_16_256 jqx16 0;}; 1: by auto.
+proc change ^while.1: { r <- sliceget256_16_256 rp0 (i0*256);};1: by auto => /#.
+proc change ^while.9: { rp0 <- sliceset256_16_256 rp0 (i0*256) r;};1: by auto => /#.
+proc change 8: { v <- sliceget16_16_256 x16p 0;}; 1: by auto.
+proc change 12: { permidx <- sliceget8_32_256 pc_permidx_s 0;}; 1: by auto.
+proc change ^while{2}.1: { f0 <- sliceget256_16_256 a (4*i*256);};1: by auto => /#.
+proc change ^while{2}.2: { f1 <- sliceget256_16_256 a ((4*i+1)*256);};1: by auto => /#.
+proc change ^while{2}.3: { f2 <- sliceget256_16_256 a ((4*i+2)*256);};1: by auto => /#.
+proc change ^while{2}.4: { f3 <- sliceget256_16_256 a ((4*i+3)*256);};1: by auto => /#.
+proc change ^while{2}.23 : { rp <- sliceset128_8_256 rp  (32*i*8) f0;};1: by auto => /#.
 
 cfold 13.
 do 2!(unroll for ^while).
 cfold ^i0<-.
 wp -3.
-bdep 16 4 [_aw] [a] [rp] compress4_circuit pcond_reduced. 
 
+
+conseq (: a = _aw /\
+   Array256.all (fun bv => W16.zero \sle bv /\ bv \slt (of_int (2 * 3329))) a
+   ==> rp = init_128_8 (fun i =>
+     W8.init (fun j =>
+       (compress4_circuit _aw.[j %/ 4 + i * 2]).[j %% 4]))); last by circuit.
+        
+       
 (* BDEP pre conseq *)
-+ move => &hr />; rewrite flatten1 /= pre_lane_commute_in_aligned 1:/# //=.
-  rewrite allP /pos_bound256_cxq /= => Hb. 
-  rewrite /pcond_reduced /= /tolist /= => x.
-  rewrite  mkseqP => He;elim He => /= i [ib?]; rewrite ultE /=.
-  have := Hb i; rewrite ib /= qE /=.
-  rewrite /to_sint /smod /=.
-  smt(W16.to_uint_cmp).
-
++ move => &hr />; rewrite /pos_bound256_cxq qE /= /(\sle) /(\slt) allP /=  => Hb i ib /=.
+  rewrite /(to_sint W16.zero) /= /(W16.smod 0) /=.
+  rewrite /(to_sint (W16.of_int 6658)) /= /(W16.smod 6658) /= /#.
+  
 (* BDEP post conseq *)
 
 (* We start with some boilerplate *)
-move => &hr [#]/= H0 <- rr; rewrite /= !flatten1.
-move => H1.
-
-apply (inj_eq Array128.to_list Array128.to_list_inj).
-apply (flatten_map_eq _ _ W8.w2bits 8 _ W8.w2bits_inj W8.size_w2bits);1:smt().
-have -> := post_lane_commute_in_aligned (to_list a{hr}) (to_list rr) W16.w2bits W16.bits2w W8.w2bits W8.bits2w W4.w2bits W4.bits2w  compress4_circuit 16 4 8 _ _ _ _ _ _ _ _ _ _ _ _ H1;1..12:
-    smt(Array128.size_to_list Array256.size_to_list W16.bits2wK BVA_Top_Bindings_W4_t.oflistP).
-
-rewrite output_pack_128_8. 
-+ rewrite (EclibExtra.size_flatten' 4);1: smt(mapP BS2Int.size_int2bs).
-  by rewrite size_map size_to_list /=.
-
-congr.
-rewrite /compress4_circuit /compress_poly -map_comp -map_comp -map_comp /(\o) /=.  
-apply (eq_from_nth witness); 1: by rewrite !size_map //.
-rewrite size_map size_iota /max /= => i ib; rewrite !(nth_map witness) //=;1,2:smt(size_iota).
-rewrite nth_iota 1:/# -(BVA_Top_Bindings_W4_t.oflistP (BS2Int.int2bs 4 (map (compress 4) (lift_array256 a{hr})).[i])); 1: by rewrite BS2Int.size_int2bs /#.
-congr; rewrite -BVA_Top_Bindings_W4_t.ofintP /lift_array256;rewrite !mapiE;1,2:smt().
-
-rewrite /truncateu4 to_uint_eq.
-(* This is now the equivalence betwen specs. It's made slightly more verbose
-   because the impl circuit is only proved correct wrt compress for values
-   in the q range. *)
-rewrite ultE /=. 
-case (to_uint a{hr}.[i] < 3329) => /= *.
-+ rewrite -compress_impl_small //=;1: by rewrite /bpos16 qE /= /to_sint /smod /=;smt(W16.to_uint_cmp).     
-  by rewrite /srl_32 /sll_32 /(`<<`) /(`>>`) !of_uintK /= /#. 
-have := H0;rewrite /pos_bound256_cxq qE /= => H00.
-
-have ? : 0 <= to_sint ((W16_sub a{hr}.[i] (W16.of_int 3329))) < 3329.
-+  rewrite /bpos16 to_sintB_small /=;1: by rewrite  /(to_sint (W16.of_int 3329)) /= /smod /=;smt(size_map size_iota). 
-   by rewrite  /(to_sint (W16.of_int 3329)) /= /smod /=; smt(size_map size_iota W16.to_uint_cmp).
-
-have ? : to_sint ((W16_sub a{hr}.[i] (W16.of_int 3329))) = to_sint a{hr}.[i] -  3329.
-+  rewrite to_sintB_small /=;1: by rewrite  /(to_sint (W16.of_int 3329))   /= /smod /=;smt(size_map size_iota). 
-   by rewrite  /(to_sint (W16.of_int 3329))  /= /smod /=; smt(size_map size_iota W16.to_uint_cmp).
-
-have -> : (incoeff (to_sint a{hr}.[i])) = (incoeff (to_sint (W16_sub a{hr}.[i] (W16.of_int 3329)))) by  rewrite -eq_incoeff;  smt().  
-
-rewrite -compress_impl_small //=;1:by smt().
-by rewrite /srl_32 /sll_32 /(`<<`) /(`>>`) !of_uintK /= /#. 
+move => &hr [#]/= H0 <- rr ->; rewrite /= /init_128_8 tP => i ib.
+rewrite wordP => k kb; rewrite !initiE 1..3:/# /=.
+rewrite encode_compress_bits //=.
+by apply compress4_circuit_sem.
 qed.
-
 (********** END BDEP PROOF OF COMPRESS **************)
 
 lemma i_poly_compress_corr _aw  : 
@@ -1180,9 +835,6 @@ qed.
 
 from JazzEC require import WArray384.
 
-op frombytes_circuit(c : W12.t) : W16.t = 
-  zeroextu16 c.
-
 
 lemma polyvec_frombytes_ll : islossless Jkem768_avx2.M.__i_polyvec_frombytes.
 proc; inline *;wp. 
@@ -1190,162 +842,22 @@ proc; inline *;wp.
 move => *. cfold 3. unroll for ^while;auto => /> /#.
 qed.
 
-op  perm_nttunpackv(i : int) : int =  nth (-1) 
-  [0; 8; 16; 24; 32; 40; 48; 56; 64; 72; 80; 88; 96; 104; 112; 120; 1; 9; 17; 25; 33; 41; 49; 57; 65; 73; 81; 89; 97;
-     105; 113; 121; 2; 10; 18; 26; 34; 42; 50; 58; 66; 74; 82; 90; 98; 106; 114; 122; 3; 11; 19; 27; 35; 43; 51; 59;
-     67; 75; 83; 91; 99; 107; 115; 123; 4; 12; 20; 28; 36; 44; 52; 60; 68; 76; 84; 92; 100; 108; 116; 124; 5; 13; 21;
-     29; 37; 45; 53; 61; 69; 77; 85; 93; 101; 109; 117; 125; 6; 14; 22; 30; 38; 46; 54; 62; 70; 78; 86; 94; 102; 110;
-     118; 126; 7; 15; 23; 31; 39; 47; 55; 63; 71; 79; 87; 95; 103; 111; 119; 127; 128; 136; 144; 152; 160; 168; 176;
-     184; 192; 200; 208; 216; 224; 232; 240; 248; 129; 137; 145; 153; 161; 169; 177; 185; 193; 201; 209; 217; 225; 233;
-     241; 249; 130; 138; 146; 154; 162; 170; 178; 186; 194; 202; 210; 218; 226; 234; 242; 250; 131; 139; 147; 155; 163;
-     171; 179; 187; 195; 203; 211; 219; 227; 235; 243; 251; 132; 140; 148; 156; 164; 172; 180; 188; 196; 204; 212; 220;
-     228; 236; 244; 252; 133; 141; 149; 157; 165; 173; 181; 189; 197; 205; 213; 221; 229; 237; 245; 253; 134; 142; 150;
-     158; 166; 174; 182; 190; 198; 206; 214; 222; 230; 238; 246; 254; 135; 143; 151; 159; 167; 175; 183; 191; 199; 207;
-     215; 223; 231; 239; 247; 255; 256; 264; 272; 280; 288; 296; 304; 312; 320; 328; 336; 344; 352; 360; 368; 376; 257;
-     265; 273; 281; 289; 297; 305; 313; 321; 329; 337; 345; 353; 361; 369; 377; 258; 266; 274; 282; 290; 298; 306; 314;
-     322; 330; 338; 346; 354; 362; 370; 378; 259; 267; 275; 283; 291; 299; 307; 315; 323; 331; 339; 347; 355; 363; 371;
-     379; 260; 268; 276; 284; 292; 300; 308; 316; 324; 332; 340; 348; 356; 364; 372; 380; 261; 269; 277; 285; 293; 301;
-     309; 317; 325; 333; 341; 349; 357; 365; 373; 381; 262; 270; 278; 286; 294; 302; 310; 318; 326; 334; 342; 350; 358;
-     366; 374; 382; 263; 271; 279; 287; 295; 303; 311; 319; 327; 335; 343; 351; 359; 367; 375; 383; 384; 392; 400; 408;
-     416; 424; 432; 440; 448; 456; 464; 472; 480; 488; 496; 504; 385; 393; 401; 409; 417; 425; 433; 441; 449; 457; 465;
-     473; 481; 489; 497; 505; 386; 394; 402; 410; 418; 426; 434; 442; 450; 458; 466; 474; 482; 490; 498; 506; 387; 395;
-     403; 411; 419; 427; 435; 443; 451; 459; 467; 475; 483; 491; 499; 507; 388; 396; 404; 412; 420; 428; 436; 444; 452;
-     460; 468; 476; 484; 492; 500; 508; 389; 397; 405; 413; 421; 429; 437; 445; 453; 461; 469; 477; 485; 493; 501; 509;
-     390; 398; 406; 414; 422; 430; 438; 446; 454; 462; 470; 478; 486; 494; 502; 510; 391; 399; 407; 415; 423; 431; 439;
-     447; 455; 463; 471; 479; 487; 495; 503; 511; 512; 520; 528; 536; 544; 552; 560; 568; 576; 584; 592; 600; 608; 616;
-     624; 632; 513; 521; 529; 537; 545; 553; 561; 569; 577; 585; 593; 601; 609; 617; 625; 633; 514; 522; 530; 538; 546;
-     554; 562; 570; 578; 586; 594; 602; 610; 618; 626; 634; 515; 523; 531; 539; 547; 555; 563; 571; 579; 587; 595; 603;
-     611; 619; 627; 635; 516; 524; 532; 540; 548; 556; 564; 572; 580; 588; 596; 604; 612; 620; 628; 636; 517; 525; 533;
-     541; 549; 557; 565; 573; 581; 589; 597; 605; 613; 621; 629; 637; 518; 526; 534; 542; 550; 558; 566; 574; 582; 590;
-     598; 606; 614; 622; 630; 638; 519; 527; 535; 543; 551; 559; 567; 575; 583; 591; 599; 607; 615; 623; 631; 639; 640;
-     648; 656; 664; 672; 680; 688; 696; 704; 712; 720; 728; 736; 744; 752; 760; 641; 649; 657; 665; 673; 681; 689; 697;
-     705; 713; 721; 729; 737; 745; 753; 761; 642; 650; 658; 666; 674; 682; 690; 698; 706; 714; 722; 730; 738; 746; 754;
-     762; 643; 651; 659; 667; 675; 683; 691; 699; 707; 715; 723; 731; 739; 747; 755; 763; 644; 652; 660; 668; 676; 684;
-     692; 700; 708; 716; 724; 732; 740; 748; 756; 764; 645; 653; 661; 669; 677; 685; 693; 701; 709; 717; 725; 733; 741;
-     749; 757; 765; 646; 654; 662; 670; 678; 686; 694; 702; 710; 718; 726; 734; 742; 750; 758; 766; 647; 655; 663; 671;
-     679; 687; 695; 703; 711; 719; 727; 735; 743; 751; 759; 767] i. 
-
-op  perm_nttpackv(i : int) =  nth (-1) 
-  [0; 16; 32; 48; 64; 80; 96; 112; 1; 17; 33; 49; 65; 81; 97; 113; 2; 18; 34; 50; 66; 82; 98; 114; 3; 19; 35; 51;
-        67; 83; 99; 115; 4; 20; 36; 52; 68; 84; 100; 116; 5; 21; 37; 53; 69; 85; 101; 117; 6; 22; 38; 54; 70; 86; 102;
-        118; 7; 23; 39; 55; 71; 87; 103; 119; 8; 24; 40; 56; 72; 88; 104; 120; 9; 25; 41; 57; 73; 89; 105; 121; 10; 26;
-        42; 58; 74; 90; 106; 122; 11; 27; 43; 59; 75; 91; 107; 123; 12; 28; 44; 60; 76; 92; 108; 124; 13; 29; 45; 61;
-        77; 93; 109; 125; 14; 30; 46; 62; 78; 94; 110; 126; 15; 31; 47; 63; 79; 95; 111; 127; 128; 144; 160; 176; 192;
-        208; 224; 240; 129; 145; 161; 177; 193; 209; 225; 241; 130; 146; 162; 178; 194; 210; 226; 242; 131; 147; 163;
-        179; 195; 211; 227; 243; 132; 148; 164; 180; 196; 212; 228; 244; 133; 149; 165; 181; 197; 213; 229; 245; 134;
-        150; 166; 182; 198; 214; 230; 246; 135; 151; 167; 183; 199; 215; 231; 247; 136; 152; 168; 184; 200; 216; 232;
-        248; 137; 153; 169; 185; 201; 217; 233; 249; 138; 154; 170; 186; 202; 218; 234; 250; 139; 155; 171; 187; 203;
-        219; 235; 251; 140; 156; 172; 188; 204; 220; 236; 252; 141; 157; 173; 189; 205; 221; 237; 253; 142; 158; 174;
-        190; 206; 222; 238; 254; 143; 159; 175; 191; 207; 223; 239; 255; 256; 272; 288; 304; 320; 336; 352; 368; 257;
-        273; 289; 305; 321; 337; 353; 369; 258; 274; 290; 306; 322; 338; 354; 370; 259; 275; 291; 307; 323; 339; 355;
-        371; 260; 276; 292; 308; 324; 340; 356; 372; 261; 277; 293; 309; 325; 341; 357; 373; 262; 278; 294; 310; 326;
-        342; 358; 374; 263; 279; 295; 311; 327; 343; 359; 375; 264; 280; 296; 312; 328; 344; 360; 376; 265; 281; 297;
-        313; 329; 345; 361; 377; 266; 282; 298; 314; 330; 346; 362; 378; 267; 283; 299; 315; 331; 347; 363; 379; 268;
-        284; 300; 316; 332; 348; 364; 380; 269; 285; 301; 317; 333; 349; 365; 381; 270; 286; 302; 318; 334; 350; 366;
-        382; 271; 287; 303; 319; 335; 351; 367; 383; 384; 400; 416; 432; 448; 464; 480; 496; 385; 401; 417; 433; 449;
-        465; 481; 497; 386; 402; 418; 434; 450; 466; 482; 498; 387; 403; 419; 435; 451; 467; 483; 499; 388; 404; 420;
-        436; 452; 468; 484; 500; 389; 405; 421; 437; 453; 469; 485; 501; 390; 406; 422; 438; 454; 470; 486; 502; 391;
-        407; 423; 439; 455; 471; 487; 503; 392; 408; 424; 440; 456; 472; 488; 504; 393; 409; 425; 441; 457; 473; 489;
-        505; 394; 410; 426; 442; 458; 474; 490; 506; 395; 411; 427; 443; 459; 475; 491; 507; 396; 412; 428; 444; 460;
-        476; 492; 508; 397; 413; 429; 445; 461; 477; 493; 509; 398; 414; 430; 446; 462; 478; 494; 510; 399; 415; 431;
-        447; 463; 479; 495; 511; 512; 528; 544; 560; 576; 592; 608; 624; 513; 529; 545; 561; 577; 593; 609; 625; 514;
-        530; 546; 562; 578; 594; 610; 626; 515; 531; 547; 563; 579; 595; 611; 627; 516; 532; 548; 564; 580; 596; 612;
-        628; 517; 533; 549; 565; 581; 597; 613; 629; 518; 534; 550; 566; 582; 598; 614; 630; 519; 535; 551; 567; 583;
-        599; 615; 631; 520; 536; 552; 568; 584; 600; 616; 632; 521; 537; 553; 569; 585; 601; 617; 633; 522; 538; 554;
-        570; 586; 602; 618; 634; 523; 539; 555; 571; 587; 603; 619; 635; 524; 540; 556; 572; 588; 604; 620; 636; 525;
-        541; 557; 573; 589; 605; 621; 637; 526; 542; 558; 574; 590; 606; 622; 638; 527; 543; 559; 575; 591; 607; 623;
-        639; 640; 656; 672; 688; 704; 720; 736; 752; 641; 657; 673; 689; 705; 721; 737; 753; 642; 658; 674; 690; 706;
-        722; 738; 754; 643; 659; 675; 691; 707; 723; 739; 755; 644; 660; 676; 692; 708; 724; 740; 756; 645; 661; 677;
-        693; 709; 725; 741; 757; 646; 662; 678; 694; 710; 726; 742; 758; 647; 663; 679; 695; 711; 727; 743; 759; 648;
-        664; 680; 696; 712; 728; 744; 760; 649; 665; 681; 697; 713; 729; 745; 761; 650; 666; 682; 698; 714; 730; 746;
-        762; 651; 667; 683; 699; 715; 731; 747; 763; 652; 668; 684; 700; 716; 732; 748; 764; 653; 669; 685; 701; 717;
-        733; 749; 765; 654; 670; 686; 702; 718; 734; 750; 766; 655; 671; 687; 703; 719; 735; 751; 767] i. 
-
-lemma perm_nttunpackv_rng i :
-  0 <= i < 768 => 0<= perm_nttunpackv i <768.
-proof.
-  have : all (fun i => 0 <= perm_nttunpackv i < 768) (iota_ 0 768).
-  + by rewrite /perm_nttunpackv  -iotaredE /=.
-  move => H Hi; rewrite allP in H; move : (H i _);by smt(mem_iota). 
-qed.
-
-lemma perm_nttpackv_rng i :
-  0 <= i < 768 => 0<= perm_nttpackv i <768.
-proof.
-  have : all (fun i => 0 <= perm_nttpackv i < 768) (iota_ 0 768).
-  + by rewrite /perm_nttpackv  -iotaredE /=.
-  move => H Hi; rewrite allP in H; move : (H i _);by smt(mem_iota). 
-qed. 
+op nttunpack_16 (rp : W16.t Array256.t) : W16.t Array256.t = init_256_16 (fun (i : int) => rp.[nttunpack_idx.[i]]).
 
 
-lemma post_lane_commute_out_aligned_perm ['a 'b 'c]
-    (lic : 'a list) 
-    (lo : 'c list) 
-    (tobitsic : 'a -> bool list)
-    (ofbitsic : bool list -> 'a)
-    (tobitsi : 'b -> bool list)
-    (ofbitsi : bool list -> 'b)
-    (tobitso : 'c -> bool list)
-    (ofbitso : bool list -> 'c)
-    (f : 'b -> 'c)
-    (nic ni no  : int) 
-    (perm : int -> int)
-    (permi : int -> int):
-  0 < nic =>  0 < ni => 0 < no => 
-  ni %| nic*size lic =>
-  size lo = (nic*size lic) %/ ni =>
-  (forall x, size (tobitsic x) = nic) =>
-  (forall x, ofbitsic (tobitsic x) = x) =>
-  (forall x, size (tobitsi x) = ni) =>
-  (forall x, ofbitsi (tobitsi x) = x) =>
-  (forall x, size x = ni => tobitsi (ofbitsi x) = x) =>
-  (forall x, size (tobitso x) = no) =>
-  (forall x, ofbitso (tobitso x) = x) =>
-  (forall ii, 0 <= ii < size lo => 0 <= perm ii < size lo) =>
-  (forall ii, 0 <= ii < size lo => permi (perm ii) = ii) =>
-map f (map ofbitsi (chunk ni (flatten (map tobitsic lic)))) =
-mkseq (fun (i1 : int) => nth witness
-(map ofbitso (chunk no (flatten (map tobitso lo)))) (permi i1)) 
-   (size (map ofbitso (chunk no (flatten (map tobitso lo))))) => 
-   lo =
-   mkseq (fun (i1 : int) => nth witness 
-      (map f (map ofbitsi (chunk ni (flatten (map tobitsic lic)))))
-         (perm i1)) (size ((map f (map ofbitsi (chunk ni (flatten (map tobitsic lic))))))).
-move => ??????????????; rewrite  !map_chunk_flatten_id 1..3:/#.
-move => H.
-apply (eq_from_nth witness).
-+ rewrite size_mkseq. 
-  rewrite !size_map size_iota (EclibExtra.size_flatten' nic);1:smt(mapP).
-  rewrite size_map; smt(size_ge0).   
-move => i ib.
-rewrite nth_mkseq /=.
-+ rewrite !size_map size_iota (EclibExtra.size_flatten' nic);1:smt(mapP).
-  rewrite size_map; smt(size_ge0).   
-rewrite H.
-rewrite nth_mkseq /=;1,2:smt().
-qed.
+op nttunpackv_16 (v : W16.t Array768.t) : W16.t Array768.t =
+  init_768_16
+    (fun (i : int) =>
+       if 0 <= i < 256 then (nttunpack_16 (subarray256 v 0)).[i]
+       else
+         if 256 <= i < 512 then (nttunpack_16 (subarray256 v 1)).[i - 256]
+         else  (nttunpack_16 (subarray256 v 2)).[i - 512]).
 
-lemma nttpermsK i :
- 0 <= i < 768 => 
-   perm_nttpackv (perm_nttunpackv i) = i.
-proof.
-move => Hi.
-have : all (fun i => perm_nttpackv (perm_nttunpackv i) = i) (iota_ 0 768); 
-  last by rewrite allP /= => H; rewrite H; smt(mem_iota).
-rewrite  /perm_nttunpackv /perm_nttpackv /nttpackv /nttunpackv.
-rewrite /nttpack /nttunpack /subarray256 -iotaredE /=;do split;smt().
-qed. 
+lemma nttunpackv_16E v: nttunpackv_16 v = nttunpackv v.
+   rewrite /nttunpackv_16 /nttunpackv /nttunpack_16 /nttunpack.
+   by rewrite /init_768_16 /init_256_16.
+   qed.
 
-lemma nttpermsKi i :
- 0 <= i < 768 => 
-   perm_nttunpackv (perm_nttpackv i) = i.
-proof.
-move => Hi.
-have : all (fun i => perm_nttunpackv (perm_nttpackv i) = i) (iota_ 0 768); 
-  last by rewrite allP /= => H; rewrite H; smt(mem_iota).
-rewrite  /perm_nttunpackv /perm_nttpackv /nttpackv /nttunpackv.
-rewrite /nttpack /nttunpack /subarray256 -iotaredE /=;do split;smt().
-qed. 
 
 lemma polyvec_frombytes_corr_h (_aw : W8.t Array1152.t): 
     hoare [Jkem768_avx2.M.__i_polyvec_frombytes  :
@@ -1354,118 +866,64 @@ lemma polyvec_frombytes_corr_h (_aw : W8.t Array1152.t):
              lift_array768 res = nttunpackv (map incoeff (decode12_vec _aw))  /\
              pos_bound768_cxq res 0 768  2].
 proc; inline *.
-proc change ^while.1: (init_256_16 (fun (i_0 : int) => r.[256 * i + i_0])); 1: by auto.
-proc change ^while.2: (init_384_8 (fun (i_0 : int) => a.[384 * i + i_0])  ); 1: by auto.
-proc change ^while.3: (sliceget16_16_256 maskx16 0); 1: by auto.
-proc change ^while.^while.1 : (sliceget384_8_256 ap (192*i0*8)); 1: by auto => /> /#.
-proc change ^while.^while.2 : (sliceget384_8_256 ap ((192*i0+32)*8)); 1: by auto => /> /#.
-proc change ^while.^while.3 : (sliceget384_8_256 ap ((192*i0+64)*8)); 1: by auto => /> /#.
-proc change ^while.^while.4 : (sliceget384_8_256 ap ((192*i0+96)*8)); 1: by auto => /> /#.
-proc change ^while.^while.5 : (sliceget384_8_256 ap ((192*i0+128)*8)); 1: by auto => /> /#.
-proc change ^while.^while.6 : (sliceget384_8_256 ap ((192*i0+160)*8)); 1: by auto => /> /#.
-proc change ^while.^while.101 : (sliceset256_16_256 rp (8*i0 *256) t6);1: by auto => /> /#.
-proc change ^while.^while.102 : (sliceset256_16_256 rp ((8*i0+1) *256) t7);1: by auto => /> /#.
-proc change ^while.^while.103 : (sliceset256_16_256 rp ((8*i0+2) *256) t8);1: by auto => /> /#.
-proc change ^while.^while.104 : (sliceset256_16_256 rp ((8*i0+3) *256) t9);1: by auto => /> /#.
-proc change ^while.^while.105 : (sliceset256_16_256 rp ((8*i0+4) *256) t4);1: by auto => /> /#.
-proc change ^while.^while.106 : (sliceset256_16_256 rp ((8*i0+5) *256) t10);1: by auto => /> /#.
-proc change ^while.^while.107 : (sliceset256_16_256 rp ((8*i0+6) *256) t11);1: by auto => /> /#.
-proc change ^while.^while.108 : (sliceset256_16_256 rp ((8*i0+7) *256) tt);1: by auto => /> /#.
-proc change ^while.7: (init_768_16 (fun (i_0 : int) => if 256 * i <= i_0 < 256 * i + 256 then aux.[i_0 - 256 * i] else r.[i_0])); 1: by auto.
+proc change ^while.1: { rp <- init_256_16 (fun (i_0 : int) => r.[256 * i + i_0]);}; 1: by auto.
+proc change ^while.2: { ap <- init_384_8 (fun (i_0 : int) => a.[384 * i + i_0]);}; 1: by auto.
+proc change ^while.3: { mask <- sliceget16_16_256 maskx16 0;}; 1: by auto.
+proc change ^while.^while.1 : { t0 <- sliceget384_8_256 ap (192*i0*8);}; 1: by auto => /> /#.
+proc change ^while.^while.2 : { t1 <- sliceget384_8_256 ap ((192*i0+32)*8);}; 1: by auto => /> /#.
+proc change ^while.^while.3 : { t2 <- sliceget384_8_256 ap ((192*i0+64)*8);}; 1: by auto => /> /#.
+proc change ^while.^while.4 : { t3 <- sliceget384_8_256 ap ((192*i0+96)*8);}; 1: by auto => /> /#.
+proc change ^while.^while.5 : { t4 <- sliceget384_8_256 ap ((192*i0+128)*8);}; 1: by auto => /> /#.
+proc change ^while.^while.6 : { t5 <- sliceget384_8_256 ap ((192*i0+160)*8);}; 1: by auto => /> /#.
+proc change ^while.^while.101 : { rp <- sliceset256_16_256 rp (8*i0 *256) t6;};1: by auto => /> /#.
+proc change ^while.^while.102 : { rp <- sliceset256_16_256 rp ((8*i0+1) *256) t7;};1: by auto => /> /#.
+proc change ^while.^while.103 : { rp <- sliceset256_16_256 rp ((8*i0+2) *256) t8;};1: by auto => /> /#.
+proc change ^while.^while.104 : { rp <- sliceset256_16_256 rp ((8*i0+3) *256) t9;};1: by auto => /> /#.
+proc change ^while.^while.105 : { rp <- sliceset256_16_256 rp ((8*i0+4) *256) t4;};1: by auto => /> /#.
+proc change ^while.^while.106 : { rp <- sliceset256_16_256 rp ((8*i0+5) *256) t10;};1: by auto => /> /#.
+proc change ^while.^while.107 : { rp <- sliceset256_16_256 rp ((8*i0+6) *256) t11;};1: by auto => /> /#.
+proc change ^while.^while.108 : { rp <- sliceset256_16_256 rp ((8*i0+7) *256) tt;};1: by auto => /> /#.
+proc change ^while.7: { r <- init_768_16 (fun (i_0 : int) => if 256 * i <= i_0 < 256 * i + 256 then aux.[i_0 - 256 * i] else r.[i_0]);}; 1: by auto.
 
 unroll for ^while.
 do 3!(unroll for ^while).
 cfold ^i0<-.
 wp -2. 
 
-bdep 12 16 [_aw] [a] [r] frombytes_circuit pcond_true12 perm_nttpackv. 
+conseq (: _ ==> r = nttunpackv_16 (init_768_16 (fun i =>
+     frombytes_circuit (
+       W12.init (fun j =>
+         let idx = i*12 + j in
+         let aidx = idx %/ 8 in
+         let bidx = idx %% 8 in
+         _aw.[aidx].[bidx]
+       )
+     )))); last by  admit. (* FIXME: TAKES TOO LONG circuit. *)
+     
+move => &hr <- rr ->.
+rewrite nttunpackv_16E;split.
++ rewrite  -nttunpackv_lift /lift_array768 /=; congr; apply Array768.tP => i ib.
+  rewrite !mapiE 1,2:/# /= initiE 1:/# /= -frombytes_circuit_sem /#.
 
-(* BDEP pre conseq *)
-+ by move => &hr />; rewrite allP /pcond_true12 /=. 
-
-(* BDEP post conseq *)
-
-(* We start with some boilerplate *)
-move => &hr [#]/= <- rr; rewrite /= !flatten1.
-
-move => H1; have H2 := post_lane_commute_out_aligned_perm (to_list a{hr}) (to_list rr) W8.w2bits W8.bits2w W12.w2bits W12.bits2w W16.w2bits W16.bits2w  frombytes_circuit 8 12 16 perm_nttunpackv perm_nttpackv _ _ _ _ _ _ _ _ _ _ _ _ _ _ _;1..12:
-smt(Array1152.size_to_list Array768.size_to_list W16.bits2wK BVA_Top_Bindings_W12_t.oflistP).
-+ smt(perm_nttunpackv_rng Array768.size_to_list).
-+ move => ?; rewrite Array768.size_to_list => ?;smt(nttpermsK). 
-
-  have /=? := decode_range_vec 0 (to_list a{hr}) 12 _ _;1,2:smt(Array1152.size_to_list).
-
-+ by smt().
-
-have H3 : 
-  map frombytes_circuit (map W12.bits2w (chunk 12 (flatten (map W8.w2bits (to_list a{hr}))))) =
-   to_list (map W16.of_int  (decode12_vec a{hr})).
-+ rewrite /decode12_vec Array768.map_of_list Array768.of_listK;1:by rewrite !size_map /decode size_iota size_BytesToBits size_to_list /#.
-  rewrite /decode -map_comp -(map_comp _ BS2Int.bs2int) /=.
-  apply eq_in_map => x xb.
-  rewrite /(\o) /frombytes_circuit /zeroextu16.
-  have ? : size x = 12 by smt(@BitChunking).
-  congr;rewrite /to_uint W12.bits2wK;1 :  by smt(@BitChunking).
-  done.
-
-split.
-+ rewrite tP => i ib.
-  rewrite mapiE 1:/# /= initiE 1:/# /=.
-  case (0<=i<256) => *.
-  + rewrite /nttunpack initiE 1:/# /= /subarray256 initiE /=;1:smt( nttunpack_inbounds).
-    rewrite mapiE /=;1:smt( nttunpack_inbounds).
-    rewrite -(Array768.get_to_list rr) H2 H3 /decode12.
-    rewrite nth_mkseq /=;1: by smt(Array768.size_to_list).
-    + rewrite  mapiE;1: by smt(perm_nttunpackv_rng).
-    congr; rewrite of_sintK /=.
-     rewrite /smod /= ifF. 
-     + rewrite /decode12_vec get_of_list;1: smt(perm_nttunpackv_rng). 
-       by have /= := decode_rng (to_list a{hr}) 12 (perm_nttunpackv i) _;smt(). 
-    rewrite modz_small. 
-    + rewrite /decode12_vec get_of_list; 1: smt(perm_nttunpackv_rng).
-       by have /= := decode_rng (to_list a{hr}) 12 (perm_nttunpackv i) _;smt(). 
-    rewrite /perm_nttunpackv /nttunpackv initiE 1:/# /= /#.
-
-  case (256<=i<512) => *.
-  + rewrite /nttunpack initiE 1:/# /= /subarray256 initiE /=;1:smt( nttunpack_inbounds).
-    rewrite mapiE /=;1:smt( nttunpack_inbounds).
-    rewrite -(Array768.get_to_list rr) H2 H3 /decode12.
-    rewrite nth_mkseq /=;1: by smt(Array768.size_to_list).
-    + rewrite  mapiE;1: by smt(perm_nttunpackv_rng).
-    congr; rewrite of_sintK /=.
-     rewrite /smod /= ifF. 
-     + rewrite /decode12_vec get_of_list;1: smt(perm_nttunpackv_rng). 
-       by have /= := decode_rng (to_list a{hr}) 12 (perm_nttunpackv i) _;smt(). 
-    rewrite modz_small. 
-    + rewrite /decode12_vec get_of_list; 1: smt(perm_nttunpackv_rng).
-       by have /= := decode_rng (to_list a{hr}) 12 (perm_nttunpackv i) _;smt(). 
-    rewrite /perm_nttunpackv /nttunpackv initiE 1:/# /= /#.
-
-
-  + rewrite /nttunpack initiE 1:/# /= /subarray256 initiE /=;1:smt( nttunpack_inbounds).
-    rewrite mapiE /=;1:smt( nttunpack_inbounds).
-    rewrite -(Array768.get_to_list rr) H2 H3 /decode12.
-    rewrite nth_mkseq /=;1: by smt(Array768.size_to_list).
-    + rewrite  mapiE;1: by smt(perm_nttunpackv_rng).
-    congr; rewrite of_sintK /=.
-     rewrite /smod /= ifF. 
-     + rewrite /decode12_vec get_of_list;1: smt(perm_nttunpackv_rng). 
-       by have /= := decode_rng (to_list a{hr}) 12 (perm_nttunpackv i) _;smt(). 
-    rewrite modz_small. 
-    + rewrite /decode12_vec get_of_list; 1: smt(perm_nttunpackv_rng).
-       by have /= := decode_rng (to_list a{hr}) 12 (perm_nttunpackv i) _;smt(). 
-    rewrite /perm_nttunpackv /nttunpackv initiE 1:/# /= /#.
-
-  rewrite /pos_bound768_cxq qE /= => k kb. 
-  have /=? := decode_range_vec witness (to_list a{hr}) 12 _ _;1..2:smt(Array1152.size_to_list).
-  rewrite -get_to_list  H2 H3 /decode12_vec.
-  rewrite nth_mkseq /=;1: by rewrite size_map size_iota /#. 
-  rewrite get_of_list;1:smt(perm_nttunpackv_rng). 
-  rewrite (nth_map witness);1:smt(perm_nttunpackv_rng). 
-rewrite of_sintK /= /smod /= ifF;1:smt(@Zq perm_nttunpackv_rng).
-  rewrite modz_small;1,2:  smt(perm_nttunpackv_rng).  
+rewrite /pos_bound768_cxq.
+move => k kb.
+have : Array768.all (fun w => bpos16 w (2*q))
+    (nttunpackv
+       (init_768_16
+          (fun (i : int) =>
+             frombytes_circuit
+               (W12.init
+                  (fun (j : int) =>
+                     let idx = i * 12 + j in let aidx = idx %/ 8 in let bidx = idx %% 8 in a{hr}.[aidx].[bidx]))))); last first.
+ + by rewrite allP => H; have /= := H k _;1:smt().
+ 
    
+apply nttunpackv_pred.
+rewrite allP => i ib; rewrite initiE 1:/# /= qE /=.
+have := frombytes_circuit_rng a{hr} i.
+smt().
 qed.
+
 
 (********** END BDEP PROOF OF FROMBYTES **************)
 
@@ -1845,10 +1303,6 @@ qed.
 
 (********** BEGIN BDEP PROOF OF FROMMSG **************)
 
-op decompress1_circuit(c : bool) : W16.t = 
-  truncateu16 (srl_32 (((if c then W32.one else W32.zero) * W32.of_int 3329) + W32.one) (W32.of_int 1)).
-
-op pcond_true (w: bool) =  true. 
 
 lemma poly_frommsg_ll : islossless Jkem768_avx2.M._i_poly_frommsg 
  by proc; inline *;wp;while (0 <= i <= 32) (32-i);  by  auto =>  /> /#.
@@ -1860,66 +1314,37 @@ lemma poly_frommsg_corr_h (_m : W8.t Array32.t):
              lift_array256 res = decompress_poly 1 (decode1 _m) /\
              pos_bound256_cxq res 0 256 1 ].
 proc; inline *.
-proc change 1: (sliceget16_16_256 hqx16_p1 0);1: by auto.
-proc change 2: (VPBROADCAST_2u128 (sliceget4_32_128 pfm_shift_s 0));1: by auto.
-proc change 3: (VPBROADCAST_2u128 (sliceget16_8_128 pfm_idx_s 0));1: by auto.
-proc change 4: (sliceget32_8_256 ap 0);1: by auto.
-proc change ^while.23 : (sliceset256_16_256 rp (2*i*256) g0); 1: by auto => /#. 
-proc change ^while.24 : (sliceset256_16_256 rp ((2*i+1)*256) g1); 1: by auto => /#. 
-proc change ^while.25 : (sliceset256_16_256 rp ((2*i+8)*256) g2); 1: by auto => /#. 
-proc change ^while.26 : (sliceset256_16_256 rp ((2*i+9)*256) g3); 1: by auto => /#. 
+proc change 1: { hqs <- sliceget16_16_256 hqx16_p1 0;};1: by auto.
+proc change 2: { shift <- VPBROADCAST_2u128 (sliceget4_32_128 pfm_shift_s 0);};1: by auto.
+proc change 3: { idx <- VPBROADCAST_2u128 (sliceget16_8_128 pfm_idx_s 0);};1: by auto.
+proc change 4: { f <- sliceget32_8_256 ap 0;};1: by auto.
+proc change ^while.23 : { rp <- sliceset256_16_256 rp (2*i*256) g0;}; 1: by auto => /#. 
+proc change ^while.24 : { rp <- sliceset256_16_256 rp ((2*i+1)*256) g1;}; 1: by auto => /#. 
+proc change ^while.25 : { rp <- sliceset256_16_256 rp ((2*i+8)*256) g2;}; 1: by auto => /#. 
+proc change ^while.26 : { rp <- sliceset256_16_256 rp ((2*i+9)*256) g3;}; 1: by auto => /#. 
 
 
 unroll for ^while.
 wp -1.
 
-bdep 1 16 [_m] [ap] [rp] decompress1_circuit pcond_true. 
 
-(* BDEP pre conseq *)
-+ by move => &hr />; rewrite allP /pcond_true /=. 
+conseq (: _ ==> rp = init_256_16 (fun i => decompress1_circuit _m.[i %/ 8].[i %% 8]));
+ 2: by circuit.
 
 (* BDEP post conseq *)
 
-(* We start with some boilerplate *)
-move => &hr [#]/= <- rr; rewrite /= !flatten1.
-move => H1; have H2 := post_lane_commute_out_aligned (to_list ap{hr}) (to_list rr) W8.w2bits W8.bits2w bool2bits bits2bool W16.w2bits W16.bits2w  decompress1_circuit 8 1 16 _ _ _ _ _ _ _ _ _ _ _ _ H1;1..12:
-smt(Array32.size_to_list Array256.size_to_list W16.bits2wK BVA_Top_Pervasive_bool.oflistP).
-
-have H3 : 
-   map decompress1_circuit (map bits2bool (chunk 1 (flatten (map W8.w2bits (to_list ap{hr}))))) =
-   map (W16.of_int \o asint) (to_list (decompress_poly 1 (decode1 ap{hr}))).
-+ rewrite /decode1 /decompress_poly Array256.map_of_list Array256.of_listK;1:smt(size_map Array256.size_to_list).
-  rewrite /decode -map_comp  -(map_comp _ (decompress 1)) -(map_comp _ BS2Int.bs2int) /=.
-  apply eq_in_map => x xb.
-  rewrite /(\o) /decompress1_circuit /bits2bool -decompress_alt_decompress /decompress_alt //=.
-  have := size_nth_chunk [] (flatten (map W8.w2bits (to_list ap{hr}))).
-  have := nthP witness (chunk 1 (flatten (map W8.w2bits (to_list ap{hr})))) x.
-  rewrite xb /= => He;elim He; rewrite size_chunk //= => k*. 
-  have ? : size x = 1 
-   by  have := size_nth_chunk witness (flatten (map W8.w2bits (to_list ap{hr}))) k 1 =>/= /#.
-  rewrite qE to_uint_eq to_uint_truncateu16 /= /srl_32 /= of_uintK /=;congr;congr.
-  rewrite to_uint_shr //=.
-  case (x = [true]).
-  + move => -> /=;rewrite bs2int_cons /= BS2Int.bs2int_nil /= /b2i /=;smt(@Zq).
-  case (x = [false]); last by smt(@List).
-  by  move => -> /=;rewrite bs2int_cons /= BS2Int.bs2int_nil /= /b2i /=;smt(@Zq).
+move => &hr [#]/= <- rr /= ->.
 
 split.
 + rewrite tP => i ib.
-  rewrite !mapiE 1,2:/# /= -get_to_list H2 H3 /decompress_poly.
-  rewrite (nth_map witness);1: by smt(Array256.size_to_list).
-  rewrite get_to_list /= /(\o) mapiE 1:/# /=.
-  pose c := (decompress 1 (decode1 ap{hr}).[i]).
-  rewrite /smod /= ifF;1:smt(@Zq).
-  rewrite modz_small; smt(@Zq).  
+  rewrite /init_256_16 !mapiE 1,2:/# /= -get_to_list /= initiE 1:/# /=.
+  by rewrite /decompress1_circuit decompress1_circuit_sem //.
 
 rewrite /pos_bound256_cxq qE /= => k kb. 
-rewrite -get_to_list  H2 H3 /decompress_poly.
-  rewrite (nth_map witness);1: by smt(Array256.size_to_list).
-  rewrite get_to_list /= /(\o) mapiE 1:/# /=.
-  rewrite  /smod /= ifF;1:smt(@Zq).
-  rewrite modz_small; smt(@Zq).  
+rewrite /init_256_16 initiE 1:/# /=.
+by smt(decompress1_circuit_rng).
 qed.
+
 
 (********** END BDEP PROOF OF FROMMSG **************)
 
@@ -1977,14 +1402,14 @@ lemma poly_tomsg_corr_h _aw :
              res.`1 = encode1 (compress_poly 1 (lift_array256 _aw))  ].
 proof.
 proc; inline *.
-proc change 3 : (sliceget16_16_256 jqx16 0);1: by auto.
-proc change ^while.1: (sliceget256_16_256 rp0 (i0*256));1: by auto => /#.
-proc change ^while.9: (sliceset256_16_256 rp0 (i0*256) r);1: by auto => /#.
-proc change 8: (sliceget16_16_256 px16 0); 1: by auto.
-proc change 10: (sliceget16_16_256 px16 0); 1: by auto.
-proc change ^while{2}.1: (sliceget256_16_256 a (2*i*256));1: by auto => /#.
-proc change ^while{2}.2: (sliceget256_16_256 a ((2*i+1)*256));1: by auto => /#.
-proc change ^while{2}.14 : (sliceset32_8_32 rp  (i*32) c);1: by auto => /#.
+proc change 3 : { qx16 <- sliceget16_16_256 jqx16 0;};1: by auto.
+proc change ^while.1: { r <- sliceget256_16_256 rp0 (i0*256);};1: by auto => /#.
+proc change ^while.9: { rp0 <- sliceset256_16_256 rp0 (i0*256) r;};1: by auto => /#.
+proc change 8: {hq <- sliceget16_16_256 px16 0;}; 1: by auto.
+proc change 10: {hhq <- sliceget16_16_256 px16 0;}; 1: by auto.
+proc change ^while{2}.1: { f0 <- sliceget256_16_256 a (2*i*256);};1: by auto => /#.
+proc change ^while{2}.2: { f1 <- sliceget256_16_256 a ((2*i+1)*256);};1: by auto => /#.
+proc change ^while{2}.14 : { rp <- sliceset32_8_32 rp  (i*32) c;};1: by auto => /#.
 
 
 cfold 11.
@@ -1993,65 +1418,22 @@ cfold ^i0<-.
 unroll for ^while.
 wp -3. 
 
-bdep 16 1 [_aw] [a] [rp] compress1_circuit pcond_reduced. 
 
-(* BDEP pre conseq *)
-+ move => &hr />; rewrite flatten1 /= pre_lane_commute_in_aligned 1:/# //=.
-  rewrite allP /pos_bound256_cxq /= => Hb. 
-  rewrite /pcond_reduced /= /tolist /= => x.
-  rewrite  mkseqP => He;elim He => /= i [ib?]; rewrite ultE /=.
-  have := Hb i; rewrite ib /= qE /=.
-  rewrite /to_sint /smod /=.
-  smt(W16.to_uint_cmp).
+conseq (: a = _aw /\
+   Array256.all (fun bv => W16.zero \sle bv /\ bv \sle (of_int (2 * 3329))) a ==> rp = init_32_8 (fun i => W8.init (fun j => compress1_circuit _aw.[i*8+j]))); last  by circuit.
+
+(* conseq pre *)
++ move => &hr />; rewrite /pos_bound256_cxq qE /= /(\sle) allP /=  => Hb i ib /=.
+  rewrite /(to_sint W16.zero) /= /(W16.smod 0) /=.
+  rewrite /(to_sint (W16.of_int 6658)) /= /(W16.smod 6658) /= /#.
 
 (* BDEP post conseq *)
-
-(* We start with some boilerplate *)
-move => &hr [#]/= H0 <- rr; rewrite /= !flatten1.
-move => H1.
-
-apply (inj_eq Array32.to_list Array32.to_list_inj).
-apply (flatten_map_eq _ _ W8.w2bits 8 _ W8.w2bits_inj W8.size_w2bits);1:smt().
-have -> := post_lane_commute_in_aligned (to_list a{hr}) (to_list rr) W16.w2bits W16.bits2w W8.w2bits W8.bits2w bool2bits bits2bool  compress1_circuit 16 1 8 _ _ _ _ _ _ _ _ _ _ _ _ H1;1..12:
-    smt(Array32.size_to_list Array256.size_to_list W16.bits2wK BVA_Top_Pervasive_bool.oflistP).
-
-rewrite output_pack_32_8. 
-+ rewrite (EclibExtra.size_flatten' 1);1: smt(mapP BS2Int.size_int2bs).
-  by rewrite size_map size_to_list /=.
-
-congr.
-rewrite /compress1_circuit /compress_poly -map_comp -map_comp -map_comp /(\o) /=.  
-apply (eq_from_nth witness); 1: by rewrite !size_map //.
-rewrite size_map size_iota /max /= => i ib; rewrite !(nth_map witness) //=;1,2:smt(size_iota).
-rewrite nth_iota 1:/# -(BVA_Top_Pervasive_bool.oflistP (BS2Int.int2bs 1 (map (compress 1) (lift_array256 a{hr})).[i]));1: by rewrite BS2Int.size_int2bs /#.
-congr; rewrite -BVA_Top_Pervasive_bool.ofintP /lift_array256;rewrite !mapiE;1,2:smt().
-
-rewrite /i2b !get_to_uint /=.
-
-(* This is now the equivalence betwen specs. It's made slightly more verbose
-   because the impl circuit is only proved correct wrt compress for values
-   in the q range. *)
-rewrite ultE /=. 
-case (to_uint a{hr}.[i] < 3329) => /= *.
-+ rewrite -compress_impl_small //=;1: by rewrite /bpos16 qE /= /to_sint /smod /=;smt(W16.to_uint_cmp).  
-  congr;congr;rewrite modz_mod;congr;congr.
-  by rewrite /srl_32 /sll_32 /(`<<`) /(`>>`).
-
-have := H0;rewrite /pos_bound256_cxq qE /= => H00.
-
-have ? : 0 <= to_sint ((W16_sub a{hr}.[i] (W16.of_int 3329))) < 3329.
-+  rewrite /bpos16 to_sintB_small /=;1: by rewrite  /(to_sint (W16.of_int 3329)) /= /smod /=;smt(size_map size_iota). 
-   by rewrite  /(to_sint (W16.of_int 3329)) /= /smod /=; smt(size_map size_iota W16.to_uint_cmp).
-
-have ? : to_sint ((W16_sub a{hr}.[i] (W16.of_int 3329))) = to_sint a{hr}.[i] -  3329.
-+  rewrite to_sintB_small /=;1: by rewrite  /(to_sint (W16.of_int 3329)) /= /smod /=;smt(size_map size_iota). 
-   by rewrite  /(to_sint (W16.of_int 3329))  /= /smod /=; smt(size_map size_iota W16.to_uint_cmp).
-
-have -> : (incoeff (to_sint a{hr}.[i])) = (incoeff (to_sint (W16_sub a{hr}.[i] (W16.of_int 3329)))) by  rewrite -eq_incoeff;  smt().  
-
-rewrite -compress_impl_small //=;1:by smt().
-by rewrite modz_mod /srl_32 /sll_32 /(`<<`) /(`>>`).
+move => &hr [#]/= H0 <- rr ->; rewrite /= /init_32_8 tP => i ib.
+rewrite wordP => k kb; rewrite !initiE 1..3:/# /=.
+rewrite encode_compress_bits //=.
+by apply compress1_circuit_sem.
 qed.
+
 
 (********** END BDEP PROOF OF TOMSG **************)
 
@@ -2078,132 +1460,11 @@ qed.
 
 (********** BEGIN BDEP PROOF OF TOBYTES **************)
 
-op tobytes_circuit(a : W16.t) : W12.t = 
-   if (a \ult W16.of_int 3329) then truncateu12 a else truncateu12 (W16_sub a (W16.of_int 3329)).  
-
 lemma polyvec_tobytes_ll : islossless Jkem768_avx2.M.__i_polyvec_tobytes.
 proc.
 inline *. 
 do 7!(unroll for ^while); auto. 
 qed.
-
-lemma post_lane_commute_in_aligned_perm ['a 'b 'c]
-    (li : 'a list) 
-    (loc : 'b list) 
-    (tobitsi : 'a -> bool list)
-    (ofbitsi : bool list -> 'a)
-    (tobitsoc : 'b -> bool list)
-    (ofbitsoc : bool list -> 'b)
-    (tobitso : 'c -> bool list)
-    (ofbitso : bool list -> 'c)
-    (f : 'a -> 'c)
-    (ni no noc  : int) 
-    (perm : int -> int)
-    (permi : int -> int):
-  0 < ni =>  0 < no => 0 < noc => 
-  no %| noc*size loc =>
-  size li = (noc*size loc) %/ no =>
-  (forall x, size (tobitsi x) = ni) =>
-  (forall x, ofbitsi (tobitsi x) = x) =>
-  (forall x, size (tobitso x) = no) =>
-  (forall x, ofbitso (tobitso x) = x) =>
-  (forall x, size x = no => tobitso (ofbitso x) = x) =>
-  (forall x, size (tobitsoc x) = noc) =>
-  (forall x, ofbitsoc (tobitsoc x) = x) =>
-  (forall ii, 0 <= ii < size li => 0 <= permi ii < size li) =>
-  (forall ii, 0 <= ii < size li => perm (permi ii) = ii) =>
-map f (map ofbitsi (chunk ni (flatten (map tobitsi  li)))) =
-mkseq (fun i => nth witness
-     (map ofbitso (chunk no (flatten (map tobitsoc loc)))) (perm i)) 
-      (size (map ofbitso (chunk no (flatten (map tobitsoc loc))))) => 
-   flatten (map tobitsoc loc) =
-   flatten (map tobitso (map f (mkseq (fun i => nth witness li (permi i)) (size li)))).
-move => 14?.
-rewrite map_chunk_flatten_id 1..3:/#.
-move => H.
-rewrite map_mkseq /(\o) /=.
-have -> : (mkseq (fun (x : int) => f (nth witness li (permi x))) (size li)) =
-   (mkseq (fun (x : int) =>  (nth witness (map f li) (permi x))) (size li)).
-+ apply eq_in_mkseq => i ib /=.
-  by rewrite (nth_map witness) 1:/#.
-rewrite H.
-have -> : (mkseq
-        (fun (x : int) =>
-           nth witness
-             (mkseq (fun (i : int) => nth witness (map ofbitso (chunk no (flatten (map tobitsoc loc)))) (perm i))
-                (size (map ofbitso (chunk no (flatten (map tobitsoc loc)))))) (
-             permi x)) (size li)) =
-   map ofbitso (mkseq
-        (fun (x : int) =>
-           nth witness
-             (mkseq (fun (i : int) => nth witness (chunk no (flatten (map tobitsoc loc))) (perm i))
-                (size (map ofbitso (chunk no (flatten (map tobitsoc loc)))))) (
-             permi x)) (size li)).
-have -> := map_mkseq ofbitso
-     (fun (x : int) =>
-        nth witness
-          (mkseq (fun (i : int) => nth witness (chunk no (flatten (map tobitsoc loc))) (perm i))
-             (size (map ofbitso (chunk no (flatten (map tobitsoc loc)))))) (
-          permi x)) (size li).
-+ apply eq_in_mkseq => i ib /=.
-  rewrite /(\o) /= !(nth_mkseq) /=;1,2: by 
-  rewrite size_map size_chunk 1:/#  (EclibExtra.size_flatten' noc);smt(mapP size_map).
-  by rewrite (nth_map witness);1: by
-   rewrite size_chunk 1:/# (EclibExtra.size_flatten' noc);smt(mapP size_map).
-
-rewrite -map_comp /(\o) /=.
-
-have -> : (mkseq
-        (fun (x : int) =>
-           nth witness
-             (mkseq (fun (i : int) => nth witness (chunk no (flatten (map tobitsoc loc))) (perm i))
-                (size (map ofbitso (chunk no (flatten (map tobitsoc loc)))))) (
-             permi x)) (size li))
- = (chunk no (flatten (map tobitsoc loc))) .
-+ apply (eq_from_nth witness).
-  + rewrite size_mkseq size_chunk 1:/# (EclibExtra.size_flatten' noc);1: smt(mapP).
-    rewrite size_map;smt(size_ge0).
-  move => i; rewrite size_mkseq /max => ib.
-  rewrite nth_mkseq 1:/# /= nth_mkseq /=.  
-  + rewrite size_map size_chunk 1:/# (EclibExtra.size_flatten' noc);1: smt(mapP).
-    rewrite size_map;smt(size_ge0).
-  by smt().
-have /= [-> x] := eq_in_map (fun (x : bool list) => tobitso (ofbitso x)) idfun (chunk no (flatten (map tobitsoc loc))).
-have := in_chunk_size no (flatten (map tobitsoc loc)) x _;smt().
-
-rewrite map_id chunkK 1:/#; last by done.
-rewrite (EclibExtra.size_flatten' noc); smt(size_map mapP).
-qed.
-
-lemma output_pack_1152_8(l : bool list) :
- size l = 768*12 =>
- flatten
-  (map W8.w2bits
-     (to_list (Array1152.of_list W8.zero (BitsToBytes l)))) = l.
-move => *.
-rewrite of_listK; 1: by rewrite size_BitsToBytes /#.
-have ? : size (flatten (map W8.w2bits (BitsToBytes l))) = size l.
-+ rewrite (EclibExtra.size_flatten' 8);1: smt(mapP W8.size_w2bits).
-  by rewrite size_map size_BitsToBytes /#.
-
-apply (eq_from_nth witness); 1: smt().
-move => i ib.
-rewrite (nth_flatten _ 8);1: by rewrite allP => *; smt( mapP W8.size_w2bits).
-rewrite (nth_map witness);1: smt(size_BitsToBytes).
-rewrite /BitsToBytes (nth_map []);1:by smt(size_chunk).
-rewrite bits2wK;1: smt(size_nth_chunk).
-rewrite -(nth_flatten _ 8);1: by rewrite allP => * /=;smt(in_chunk_size). 
-by rewrite chunkK /#.
-qed.
-
-lemma nttpackv_alt (a : W16.t Array768.t) i :
- 0 <= i < 768 =>
-  a.[perm_nttpackv i] = (nttpackv a).[i].
-proof.
-move => ?;have : all (fun i => a.[perm_nttpackv i] = (nttpackv a).[i]) (iota_ 0 768);
-  last by rewrite allP => H; move : (H i);smt(mem_iota).
-by rewrite /nttpackv /subarray256 /nttpack /perm_nttpackv -iotaredE /=.
-qed. 
 
 abbrev mask12 = VPBROADCAST_16u16(W16.of_int 4095).
 
@@ -2357,33 +1618,50 @@ proc __i_polyvec_tobytes(r : W8.t Array1152.t, a : W16.t Array768.t) : W8.t Arra
  }       
 }.
 
+op nttpack_16 (rp : W16.t Array256.t)  = init_256_16 (fun (i : int) => rp.[nttpack_idx.[i]]).
+
+op nttpackv_16 (v : W16.t Array768.t) =
+  init_768_16
+    (fun (i : int) =>
+       if 0 <= i < 256 then (nttpack_16 (subarray256 v 0)).[i]
+       else
+         if 256 <= i < 512 then (nttpack_16 (subarray256 v 1)).[i - 256]
+         else  (nttpack_16 (subarray256 v 2)).[i - 512]).
+
+lemma nttpackv_16E v : nttpackv_16 v = nttpackv v.
+rewrite /nttpackv_16 /init_768_16 /nttpack_16 /init_256_16.
+by rewrite /nttpackv /nttpack.
+qed.
+
+
+
 lemma auxtobytes_corr_h (_aw : W16.t Array768.t):
     hoare[AuxToBytes.__i_polyvec_tobytes :
              pos_bound768_cxq a 0 768 2 /\ a = _aw ==> 
     res = encode12_vec (map asint (lift_array768 (nttpackv _aw)))]. 
 proc;inline *.
-proc change ^while.1: (init_384_8 (fun i_0 => r.[384 * i + i_0]));1: by auto.
-proc change ^while.2: (init_256_16 (fun i_0 => a.[256 * i + i_0]));1: by auto.
+proc change ^while.1: {rp <- init_384_8 (fun i_0 => r.[384 * i + i_0]);};1: by auto.
+proc change ^while.2: {a0 <- init_256_16 (fun i_0 => a.[256 * i + i_0]);};1: by auto.
 (* FIXME: CHECK qx16 initialization inside while *)
-proc change ^while.4: (sliceget16_16_256 jqx16 0); 1: by auto.
-proc change ^while.^while.1: (sliceget256_16_256 rp0 (i1*256)); 1: by auto => /#.
-proc change ^while.^while.9 : (sliceset256_16_256 rp0 (i1*256) r0); 1: by auto => /> /#.
-proc change ^while.^while{2}.1 : (sliceget256_16_256 a0 (8*i0*256));1: by auto => /#.
-proc change ^while.^while{2}.2 : (sliceget256_16_256 a0 ((8*i0+1)*256));1: by auto => /#.
-proc change ^while.^while{2}.3 : (sliceget256_16_256 a0 ((8*i0+2)*256));1: by auto => /#.
-proc change ^while.^while{2}.4 : (sliceget256_16_256 a0 ((8*i0+3)*256));1: by auto => /#.
-proc change ^while.^while{2}.5 : (sliceget256_16_256 a0 ((8*i0+4)*256));1: by auto => /#.
-proc change ^while.^while{2}.6 : (sliceget256_16_256 a0 ((8*i0+5)*256));1: by auto => /#.
-proc change ^while.^while{2}.7 : (sliceget256_16_256 a0 ((8*i0+6)*256));1: by auto => /#.
-proc change ^while.^while{2}.8 : (sliceget256_16_256 a0 ((8*i0+7)*256));1: by auto => /#.
-proc change ^while.^while{2}.105 : (sliceset384_8_256 rp (192*i0*8) t0);1: by auto => /#.
-proc change ^while.^while{2}.106 : (sliceset384_8_256 rp ((192*i0+32)*8) t2);1: by auto => /#.
-proc change ^while.^while{2}.107 : (sliceset384_8_256 rp ((192*i0+64)*8) t1);1: by auto => /#.
-proc change ^while.^while{2}.108 : (sliceset384_8_256 rp ((192*i0+96)*8) t3);1: by auto => /#.
-proc change ^while.^while{2}.109 : (sliceset384_8_256 rp ((192*i0+128)*8) ttt);1: by auto => /#.
-proc change ^while.^while{2}.110 : (sliceset384_8_256 rp ((192*i0+160)*8) t4);1: by auto => /#.
-proc change ^while.11: (init_1152_8 (fun (i_0 : int) => if 384 * i <= i_0 < 384 * i + 384 then aux.[i_0 - 384 * i] else r.[i_0])  ); 1: by auto.
-proc change ^while.12: (init_768_16  (fun (i_0 : int) => if 256 * i <= i_0 < 256 * i + 256 then aux_0.[i_0 - 256 * i] else a.[i_0]));1: by auto. 
+proc change ^while.4: {qx16 <- sliceget16_16_256 jqx16 0;}; 1: by auto.
+proc change ^while.^while.1: { r0 <- sliceget256_16_256 rp0 (i1*256);}; 1: by auto => /#.
+proc change ^while.^while.9 : {rp0 <- sliceset256_16_256 rp0 (i1*256) r0;}; 1: by auto => /> /#.
+proc change ^while.^while{2}.1 : {t0 <- sliceget256_16_256 a0 (8*i0*256);};1: by auto => /#.
+proc change ^while.^while{2}.2 : {t1 <- sliceget256_16_256 a0 ((8*i0+1)*256);};1: by auto => /#.
+proc change ^while.^while{2}.3 : {t2 <- sliceget256_16_256 a0 ((8*i0+2)*256);};1: by auto => /#.
+proc change ^while.^while{2}.4 : {t3 <- sliceget256_16_256 a0 ((8*i0+3)*256);};1: by auto => /#.
+proc change ^while.^while{2}.5 : {t4 <- sliceget256_16_256 a0 ((8*i0+4)*256);};1: by auto => /#.
+proc change ^while.^while{2}.6 : {t5 <- sliceget256_16_256 a0 ((8*i0+5)*256);};1: by auto => /#.
+proc change ^while.^while{2}.7 : {t6 <- sliceget256_16_256 a0 ((8*i0+6)*256);};1: by auto => /#.
+proc change ^while.^while{2}.8 : {t7 <- sliceget256_16_256 a0 ((8*i0+7)*256);};1: by auto => /#.
+proc change ^while.^while{2}.105 : {rp <- sliceset384_8_256 rp (192*i0*8) t0;};1: by auto => /#.
+proc change ^while.^while{2}.106 : {rp <- sliceset384_8_256 rp ((192*i0+32)*8) t2;};1: by auto => /#.
+proc change ^while.^while{2}.107 : {rp <- sliceset384_8_256 rp ((192*i0+64)*8) t1;};1: by auto => /#.
+proc change ^while.^while{2}.108 : {rp <- sliceset384_8_256 rp ((192*i0+96)*8) t3;};1: by auto => /#.
+proc change ^while.^while{2}.109 : {rp <- sliceset384_8_256 rp ((192*i0+128)*8) ttt;};1: by auto => /#.
+proc change ^while.^while{2}.110 : {rp <- sliceset384_8_256 rp ((192*i0+160)*8) t4;};1: by auto => /#.
+proc change ^while.11: { r <- init_1152_8 (fun (i_0 : int) => if 384 * i <= i_0 < 384 * i + 384 then aux.[i_0 - 384 * i] else r.[i_0]);}; 1: by auto.
+proc change ^while.12: { a <- init_768_16  (fun (i_0 : int) => if 256 * i <= i_0 < 256 * i + 256 then aux_0.[i_0 - 256 * i] else a.[i_0]);};1: by auto. 
 
 unroll for ^while.
 do 6!(unroll for ^while).
@@ -2392,66 +1670,31 @@ cfold ^i0<-.
 cfold ^i1<-.
 wp -3.
 
-bdep 16 12 [_aw] [a] [r] tobytes_circuit pcond_reduced perm_nttunpackv. 
 
-(* BDEP pre conseq *)
-+ move => &hr />; rewrite flatten1 /= pre_lane_commute_in_aligned 1:/# //=.
-  rewrite allP /pos_bound768_cxq /= => Hb. 
-  rewrite /pcond_reduced /= /tolist /= => x.
-  rewrite  mkseqP => He;elim He => /= i [ib?]; rewrite ultE /=.
-  have := Hb i; rewrite ib /= qE /=.
-  rewrite /to_sint /smod /=.
-  smt(W16.to_uint_cmp).
+conseq (: 
+ a = _aw /\
+   Array768.all (fun bv => W16.zero \sle bv /\ bv \slt (of_int (2 * 3329))) a
+   ==> r =  let ret = init_768_12 (fun j => tobytes_circuit (nttpackv_16 _aw).[j]) in
+  init_1152_8 (fun i =>
+    W8.init (fun j =>
+      let idx = i*8 + j in
+      let aidx = idx %/ 12 in
+      let bidx = idx %% 12 in
+      W12."_.[_]" (ret.[aidx]) bidx))); last by admit. (* FIXME: takes too long *)
+      
++ move => &hr />; rewrite allP /= /pos_bound768_cxq /(\sle) /(\slt) /= /qE /smod /=.
+  by rewrite qE /= => H k ?; move : (H k _) => //=.
 
-(* BDEP post conseq *)
+move => &hr [#]/=; rewrite /pos_bound768_cxq /bpos16 => H0 <- rr ->.
+rewrite /init_1152_8 /encode12 tP => i ib.
+rewrite initiE 1:/# /= get_of_list 1:/# /= wordP => k kb.
+rewrite initiE //= /init_256_12 initiE 1:/# /=.
+have := nttpackv_pred a{hr} (fun c => bpos16 c (2 * q)).
+rewrite !allP  /= iffE qE /= => [#_ H].
+by rewrite nttpackv_16E  to_bytes_circuit_sem;1..3:
+ by rewrite /(\ult) /=; smt(W16.to_sint_unsigned).
+ qed.
 
-(* We start with some boilerplate *)
-move => &hr [#]/= H0 <- rr; rewrite /= !flatten1.
-move => H1.
-apply (inj_eq Array1152.to_list Array1152.to_list_inj).
-apply (flatten_map_eq _ _ W8.w2bits 8 _ W8.w2bits_inj W8.size_w2bits);1:smt().
-have -> := post_lane_commute_in_aligned_perm (to_list a{hr}) (to_list rr) W16.w2bits W16.bits2w W8.w2bits W8.bits2w W12.w2bits W12.bits2w  tobytes_circuit 16 12 8 perm_nttunpackv perm_nttpackv _ _ _ _ _ _ _ _ _ _ _ _ _ _ _;1..12:
-smt(Array1152.size_to_list Array768.size_to_list W16.bits2wK BVA_Top_Bindings_W12_t.oflistP).
-+ smt(perm_nttpackv_rng Array768.size_to_list).
-+ move => ?; rewrite Array768.size_to_list => ?;smt(nttpermsKi). 
-+ by smt().
-
-rewrite output_pack_1152_8. 
-+ rewrite (EclibExtra.size_flatten' 12);1: smt(mapP BS2Int.size_int2bs).
-  by rewrite size_map size_to_list /=.
-
-congr.
-rewrite /tobytes_circuit -map_comp -map_comp -map_comp /(\o) /=.
-apply (eq_from_nth witness);1: by  rewrite !size_map //;smt(size_iota).
-rewrite size_map !size_iota /max /= => i; rewrite size_to_list /= => ib; rewrite !(nth_map witness) //=;1,2:smt(size_iota).
-rewrite nth_iota 1:/# -(BVA_Top_Bindings_W12_t.oflistP (BS2Int.int2bs 12 (map asint (lift_array768 (nttpackv a{hr}))).[i])); 1: by rewrite BS2Int.size_int2bs /#.
-congr; rewrite -BVA_Top_Bindings_W12_t.ofintP /lift_array256;rewrite !mapiE 1,2:/#.
-
-(* This is now the equivalence betwen specs.*)
-rewrite ultE /=; have HH := nttpackv_alt a{hr} i ib.
-have HG := perm_nttpackv_rng i ib.
-rewrite HH.
-
-case (to_uint (nttpackv a{hr}).[i] < 3329) => /= *.
-+ rewrite  /truncateu12;congr. 
-  rewrite incoeffK qE /to_sint /= /smod /= ifF 1:/#  modz_small;smt(W16.to_uint_cmp). 
-
-have := H0;rewrite /pos_bound768_cxq qE /= => H00.
-
-have ? : 0 <= to_sint ((W16_sub (nttpackv a{hr}).[i] (W16.of_int 3329))) < 3329.
-+  rewrite /bpos16 to_sintB_small /=;1: by rewrite  /(to_sint (W16.of_int 3329))  /= /smod /=;smt(size_map size_iota). 
-   rewrite  /(to_sint (W16.of_int 3329)) /= /smod /=;   smt(size_map size_iota W16.to_uint_cmp).
-
-have ? : to_sint ((W16_sub (nttpackv a{hr}).[i] (W16.of_int 3329))) = to_sint (nttpackv a{hr}).[i] -  3329.
-+  rewrite to_sintB_small /=;1: by rewrite  /(to_sint (W16.of_int 3329))  /= /smod /=;smt(size_map size_iota). 
-   by rewrite  /(to_sint (W16.of_int 3329))  /= /smod /=; smt(size_map size_iota W16.to_uint_cmp).
-
-have -> : (incoeff (to_sint (nttpackv a{hr}).[i])) = (incoeff (to_sint (W16_sub (nttpackv a{hr}).[i] (W16.of_int 3329)))) by  rewrite -eq_incoeff; smt(). 
-
-+ rewrite  /truncateu12;congr. 
-  rewrite incoeffK qE modz_small;smt(W16.to_uint_cmp). 
- 
-qed.
 
 lemma auxtobytes_ll : islossless AuxToBytes.__i_polyvec_tobytes.
 proc.
