proof/correctness768/MLKEM_Poly.ec
@@ -402,7 +402,7 @@ lemma poly_frommont_corr (_a : int Array256.t) :
     phoare[Jkem768.M._poly_frommont :
              forall k, 0<=k<256 => to_sint rp.[k] = _a.[k] ==>
              forall k, 0<=k<256 => to_sint res.[k] = SREDC (_a.[k] * ((R^2) %% q))]=1%r
-        by admit. (* conseq poly_frommont_ll  (poly_frommont_corr_h _a). *)
+        by  conseq poly_frommont_ll  (poly_frommont_corr_h _a). 
 
 lemma poly_sub_corr_h _a _b ab bb :
     0 <= ab <= 4 => 0 <= bb <= 4 =>  
@@ -455,7 +455,7 @@ lemma poly_sub_corr _a _b ab bb :
            signed_bound_cxq res 0 256 (ab + bb) /\ 
            forall k, 0 <= k < 256 =>
               incoeff (to_sint res.[k]) = _a.[k] - _b.[k]] = 1%r 
-   by admit. (* move => *;conseq poly_sub_ll (poly_sub_corr_h _a _b ab bb _ _). *)
+   by  move => *;conseq poly_sub_ll (poly_sub_corr_h _a _b ab bb _ _). 
 
 lemma poly_sub_corr_alg ab bb :
   0 <= ab <= 4 =>
@@ -537,7 +537,7 @@ lemma poly_add_corr _a _b ab bb :
            signed_bound_cxq res 0 256 (ab + bb) /\ 
            forall k, 0 <= k < 256 =>
               incoeff (to_sint res.[k]) = _a.[k] + _b.[k]] = 1%r
-   by admit. (* move => abb bbb; conseq poly_add_ll (poly_add_corr_h _a _b ab bb abb bbb).  *)
+   by  move => abb bbb; conseq poly_add_ll (poly_add_corr_h _a _b ab bb abb bbb).  
 
 lemma poly_add_corr_impl_h ab bb :
   0 <= ab <= 6 =>
@@ -593,7 +593,7 @@ lemma poly_add_correct_impl ab bb :
            signed_bound_cxq res 0 256 (ab + bb) /\ 
            forall k, 0 <= k < 256 =>
               incoeff (to_sint res.[k]) = _a.[k] + _b.[k]] = 1%r
-   by admit. (* move => abb bbb _a _b; conseq poly_add_ll (poly_add_corr_impl_h ab bb abb bbb _a _b ). *)
+   by  move => abb bbb _a _b; conseq poly_add_ll (poly_add_corr_impl_h ab bb abb bbb _a _b ). 
 
 
 lemma poly_reduce_corr_h (_a : coeff Array256.t):
@@ -646,7 +646,7 @@ lemma poly_reduce_corr (_a : coeff Array256.t):
           _a = lift_array256 rp ==> 
           _a = lift_array256 res /\
           forall k, 0 <= k < 256 => bpos16  res.[k] (2*q)] = 1%r
-          by admit. (* conseq poly_reduce_ll (poly_reduce_corr_h _a). qed. *)
+          by  conseq poly_reduce_ll (poly_reduce_corr_h _a).  
 
 (********** BEGIN BDEP PROOF OF TOBYTES **************)
 
